<?xml version="1.0"?>
<rdf:RDF xmlns="https://purls.helmholtz-metadaten.de/disos/diso"
     xml:base="https://purls.helmholtz-metadaten.de/disos/diso"
     xmlns:owl="http://www.w3.org/2002/07/owl#"
     xmlns:rdf="http://www.w3.org/1999/02/22-rdf-syntax-ns#"
     xmlns:xml="http://www.w3.org/XML/1998/namespace"
     xmlns:xsd="http://www.w3.org/2001/XMLSchema#"
     xmlns:qudt="http://qudt.org/schema/qudt/"
     xmlns:rdfs="http://www.w3.org/2000/01/rdf-schema#"
     xmlns:skos="http://www.w3.org/2004/02/skos/core#"
     xmlns:vann="http://purl.org/vocab/vann/"
     xmlns:terms="http://purl.org/dc/terms/">
    <owl:Ontology rdf:about="https://purls.helmholtz-metadaten.de/disos/diso">
        <owl:imports rdf:resource="https://w3id.org/mdo/core/1.1/"/>
        <terms:contributor rdf:datatype="http://www.w3.org/2001/XMLSchema#string">Said Fathalla</terms:contributor>
        <terms:contributor rdf:datatype="http://www.w3.org/2001/XMLSchema#string">Stefan Sandfeld</terms:contributor>
        <terms:created xml:lang="en">21.03.2022</terms:created>
        <terms:creator xml:lang="en">Ahmad Zainul Ihsan</terms:creator>
        <terms:license rdf:resource="http://creativecommons.org/licenses/by/3.0/"/>
        <terms:title xml:lang="en">Dislocation Ontology</terms:title>
        <vann:preferredNamespacePrefix rdf:datatype="http://www.w3.org/2001/XMLSchema#string">DISO</vann:preferredNamespacePrefix>
        <rdfs:label xml:lang="en">Dislocation Ontology</rdfs:label>
        <rdfs:seeAlso>https://github.com/Materials-Data-Science-and-Informatics/dislocation-ontology</rdfs:seeAlso>
        <owl:versionInfo rdf:datatype="http://www.w3.org/2001/XMLSchema#decimal">1.1</owl:versionInfo>
    </owl:Ontology>
    


    <!-- 
    ///////////////////////////////////////////////////////////////////////////////////////
    //
    // Annotation properties
    //
    ///////////////////////////////////////////////////////////////////////////////////////
     -->

    


    <!-- http://purl.org/dc/terms/contributor -->

    <owl:AnnotationProperty rdf:about="http://purl.org/dc/terms/contributor"/>
    


    <!-- http://purl.org/dc/terms/created -->

    <owl:AnnotationProperty rdf:about="http://purl.org/dc/terms/created"/>
    


    <!-- http://purl.org/dc/terms/creator -->

    <owl:AnnotationProperty rdf:about="http://purl.org/dc/terms/creator"/>
    


    <!-- http://purl.org/dc/terms/license -->

    <owl:AnnotationProperty rdf:about="http://purl.org/dc/terms/license"/>
    


    <!-- http://purl.org/dc/terms/title -->

    <owl:AnnotationProperty rdf:about="http://purl.org/dc/terms/title"/>
    


    <!-- http://purl.org/vocab/vann/preferredNamespacePrefix -->

    <owl:AnnotationProperty rdf:about="http://purl.org/vocab/vann/preferredNamespacePrefix"/>
    


    <!-- http://qudt.org/schema/qudt/description -->

    <owl:AnnotationProperty rdf:about="http://qudt.org/schema/qudt/description"/>
    


    <!-- http://www.w3.org/2004/02/skos/core#defintion -->

    <owl:AnnotationProperty rdf:about="http://www.w3.org/2004/02/skos/core#defintion"/>
    


    <!-- http://www.w3.org/2004/02/skos/core#prefLabel -->

    <owl:AnnotationProperty rdf:about="http://www.w3.org/2004/02/skos/core#prefLabel"/>
    


    <!-- 
    ///////////////////////////////////////////////////////////////////////////////////////
    //
    // Datatypes
    //
    ///////////////////////////////////////////////////////////////////////////////////////
     -->

    


    <!-- http://www.w3.org/1999/02/22-rdf-syntax-ns#HTML -->

    <rdfs:Datatype rdf:about="http://www.w3.org/1999/02/22-rdf-syntax-ns#HTML"/>
    


    <!-- 
    ///////////////////////////////////////////////////////////////////////////////////////
    //
    // Object Properties
    //
    ///////////////////////////////////////////////////////////////////////////////////////
     -->

    


    <!-- http://emmo.info/emmo#EMMO_e1097637_70d2_4895_973f_2396f04fa204 -->

    <owl:ObjectProperty rdf:about="http://emmo.info/emmo#EMMO_e1097637_70d2_4895_973f_2396f04fa204">
        <skos:prefLabel xml:lang="en">hasProperty</skos:prefLabel>
    </owl:ObjectProperty>
    


    <!-- http://qudt.org/schema/qudt/hasQuantityKind -->

    <owl:ObjectProperty rdf:about="http://qudt.org/schema/qudt/hasQuantityKind"/>
    


    <!-- http://qudt.org/schema/qudt/quantityValue -->

    <owl:ObjectProperty rdf:about="http://qudt.org/schema/qudt/quantityValue"/>
    


    <!-- http://qudt.org/schema/qudt/unit -->

    <owl:ObjectProperty rdf:about="http://qudt.org/schema/qudt/unit"/>
    


    <!-- http://www.w3.org/ns/prov#wasAssociatedWith -->

    <owl:ObjectProperty rdf:about="http://www.w3.org/ns/prov#wasAssociatedWith"/>
    


    <!-- https://purls.helmholtz-metadaten.de/disos/cdo#hasCrystalStructure -->

    <owl:ObjectProperty rdf:about="https://purls.helmholtz-metadaten.de/disos/cdo#hasCrystalStructure">
        <rdfs:label>has crystal structure</rdfs:label>
    </owl:ObjectProperty>
    


    <!-- https://purls.helmholtz-metadaten.de/disos/cdo#hasCrystallographicDefect -->

    <owl:ObjectProperty rdf:about="https://purls.helmholtz-metadaten.de/disos/cdo#hasCrystallographicDefect">
        <rdfs:domain>
            <owl:Class>
                <owl:unionOf rdf:parseType="Collection">
                    <rdf:Description rdf:about="https://purls.helmholtz-metadaten.de/disos/cdo#CrystallineMaterial"/>
                    <rdf:Description rdf:about="https://purls.helmholtz-metadaten.de/disos/diso#DislocationStructure"/>
                </owl:unionOf>
            </owl:Class>
        </rdfs:domain>
        <rdfs:range rdf:resource="https://purls.helmholtz-metadaten.de/disos/cdo#CrystallographicDefect"/>
        <rdfs:label>has crystallographic defect</rdfs:label>
    </owl:ObjectProperty>
    


    <!-- https://purls.helmholtz-metadaten.de/disos/cso#hasBasis -->

    <owl:ObjectProperty rdf:about="https://purls.helmholtz-metadaten.de/disos/cso#hasBasis"/>
    


    <!-- https://purls.helmholtz-metadaten.de/disos/cso#hasFirstAxisVector -->

    <owl:ObjectProperty rdf:about="https://purls.helmholtz-metadaten.de/disos/cso#hasFirstAxisVector"/>
    


    <!-- https://purls.helmholtz-metadaten.de/disos/cso#hasPositionVector -->

    <owl:ObjectProperty rdf:about="https://purls.helmholtz-metadaten.de/disos/cso#hasPositionVector">
        <rdfs:domain rdf:resource="https://purls.helmholtz-metadaten.de/disos/cso#Point"/>
        <rdfs:range rdf:resource="https://purls.helmholtz-metadaten.de/disos/cso#PositionVector"/>
        <rdfs:comment xml:lang="en">hasPositionVector represents the relationship between entity and position vector.</rdfs:comment>
        <rdfs:label xml:lang="en">has position vector</rdfs:label>
    </owl:ObjectProperty>
    


    <!-- https://purls.helmholtz-metadaten.de/disos/cso#hasSecondAxisVector -->

    <owl:ObjectProperty rdf:about="https://purls.helmholtz-metadaten.de/disos/cso#hasSecondAxisVector"/>
    


    <!-- https://purls.helmholtz-metadaten.de/disos/cso#hasThirdAxisVector -->

    <owl:ObjectProperty rdf:about="https://purls.helmholtz-metadaten.de/disos/cso#hasThirdAxisVector"/>
    


    <!-- https://purls.helmholtz-metadaten.de/disos/cso#hasVectorComponent -->

    <owl:ObjectProperty rdf:about="https://purls.helmholtz-metadaten.de/disos/cso#hasVectorComponent"/>
    


    <!-- https://purls.helmholtz-metadaten.de/disos/diso#hasBurgersVector -->

    <owl:ObjectProperty rdf:about="https://purls.helmholtz-metadaten.de/disos/diso#hasBurgersVector">
        <rdfs:domain rdf:resource="https://purls.helmholtz-metadaten.de/disos/diso#Dislocation"/>
        <rdfs:range rdf:resource="https://purls.helmholtz-metadaten.de/disos/diso#BurgersVector"/>
        <rdfs:comment xml:lang="en">hasBurgersVector represents the relationship between dislocation to Burgers vector.</rdfs:comment>
        <rdfs:label xml:lang="en">has Burgers vector</rdfs:label>
    </owl:ObjectProperty>
    


    <!-- https://purls.helmholtz-metadaten.de/disos/diso#hasEndNode -->

    <owl:ObjectProperty rdf:about="https://purls.helmholtz-metadaten.de/disos/diso#hasEndNode">
        <rdfs:subPropertyOf rdf:resource="https://purls.helmholtz-metadaten.de/disos/diso#hasNode"/>
        <rdfs:domain rdf:resource="https://purls.helmholtz-metadaten.de/disos/diso#Segment"/>
        <rdfs:range rdf:resource="https://purls.helmholtz-metadaten.de/disos/diso#Node"/>
        <rdfs:comment xml:lang="en">Sub-property of hasNode that relates the segment with the end node.</rdfs:comment>
        <rdfs:label xml:lang="en">has end node</rdfs:label>
    </owl:ObjectProperty>
    


    <!-- https://purls.helmholtz-metadaten.de/disos/diso#hasFamilyCrystalDirection -->

    <owl:ObjectProperty rdf:about="https://purls.helmholtz-metadaten.de/disos/diso#hasFamilyCrystalDirection">
        <rdfs:domain rdf:resource="https://purls.helmholtz-metadaten.de/disos/diso#LatticeDirection"/>
        <rdfs:range rdf:resource="https://purls.helmholtz-metadaten.de/disos/diso#FamilyOfCrystalDirection"/>
        <rdfs:comment xml:lang="en">hasFamilyCrystalDirection represents the relationship between lattice direction and family of crystal direction.</rdfs:comment>
        <rdfs:label xml:lang="en">has family crystal direction</rdfs:label>
    </owl:ObjectProperty>
    


    <!-- https://purls.helmholtz-metadaten.de/disos/diso#hasFamilyCrystalPlane -->

    <owl:ObjectProperty rdf:about="https://purls.helmholtz-metadaten.de/disos/diso#hasFamilyCrystalPlane">
        <rdfs:domain rdf:resource="https://purls.helmholtz-metadaten.de/disos/diso#LatticePlane"/>
        <rdfs:range rdf:resource="https://purls.helmholtz-metadaten.de/disos/diso#FamilyOfCrystalPlane"/>
        <rdfs:comment xml:lang="en">hasFamilyCrystalPlane represents the relationship between the lattice plane and the family of crystal planes.</rdfs:comment>
        <rdfs:label xml:lang="en">has family crystal plane</rdfs:label>
    </owl:ObjectProperty>
    


    <!-- https://purls.helmholtz-metadaten.de/disos/diso#hasInputDislocationStructure -->

    <owl:ObjectProperty rdf:about="https://purls.helmholtz-metadaten.de/disos/diso#hasInputDislocationStructure">
        <rdfs:subPropertyOf rdf:resource="https://w3id.org/mdo/core/hasInputStructure"/>
        <rdfs:domain rdf:resource="https://purls.helmholtz-metadaten.de/disos/diso#DDDSimulation"/>
        <rdfs:range rdf:resource="https://purls.helmholtz-metadaten.de/disos/diso#DislocationStructure"/>
        <rdfs:label xml:lang="en">has input dislocation structure</rdfs:label>
    </owl:ObjectProperty>
    


    <!-- https://purls.helmholtz-metadaten.de/disos/diso#hasLatticeDirection -->

    <owl:ObjectProperty rdf:about="https://purls.helmholtz-metadaten.de/disos/diso#hasLatticeDirection">
        <rdfs:domain>
            <owl:Class>
                <owl:unionOf rdf:parseType="Collection">
                    <rdf:Description rdf:about="https://purls.helmholtz-metadaten.de/disos/cso#Lattice"/>
                    <rdf:Description rdf:about="https://purls.helmholtz-metadaten.de/disos/diso#LatticePlane"/>
                </owl:unionOf>
            </owl:Class>
        </rdfs:domain>
        <rdfs:range rdf:resource="https://purls.helmholtz-metadaten.de/disos/diso#LatticeDirection"/>
        <rdfs:comment xml:lang="en">hasLatticeDirection represents the relationship between a lattice or a lattice plane with lattice directions.</rdfs:comment>
        <rdfs:label xml:lang="en">has lattice direction</rdfs:label>
    </owl:ObjectProperty>
    


    <!-- https://purls.helmholtz-metadaten.de/disos/diso#hasLatticePlane -->

    <owl:ObjectProperty rdf:about="https://purls.helmholtz-metadaten.de/disos/diso#hasLatticePlane">
        <rdfs:domain>
            <owl:Class>
                <owl:unionOf rdf:parseType="Collection">
                    <rdf:Description rdf:about="https://purls.helmholtz-metadaten.de/disos/cso#CrystalStructure"/>
                    <rdf:Description rdf:about="https://purls.helmholtz-metadaten.de/disos/cso#Lattice"/>
                </owl:unionOf>
            </owl:Class>
        </rdfs:domain>
        <rdfs:range rdf:resource="https://purls.helmholtz-metadaten.de/disos/diso#LatticePlane"/>
        <rdfs:comment xml:lang="en">hasLatticePlane represents the relationship between a lattice and lattice planes.</rdfs:comment>
        <rdfs:label xml:lang="en">has lattice plane</rdfs:label>
    </owl:ObjectProperty>
    


    <!-- https://purls.helmholtz-metadaten.de/disos/diso#hasLatticePoint -->

    <owl:ObjectProperty rdf:about="https://purls.helmholtz-metadaten.de/disos/diso#hasLatticePoint">
        <rdfs:domain>
            <owl:Class>
                <owl:unionOf rdf:parseType="Collection">
                    <rdf:Description rdf:about="https://purls.helmholtz-metadaten.de/disos/cso#Lattice"/>
                    <rdf:Description rdf:about="https://purls.helmholtz-metadaten.de/disos/diso#LatticeDirection"/>
                    <rdf:Description rdf:about="https://purls.helmholtz-metadaten.de/disos/diso#LatticePlane"/>
                </owl:unionOf>
            </owl:Class>
        </rdfs:domain>
        <rdfs:range rdf:resource="https://purls.helmholtz-metadaten.de/disos/diso#LatticePoint"/>
        <rdfs:comment xml:lang="en">hasLatticePoint represents the relationship between a lattice or lattice plane or lattice direction with lattice point.</rdfs:comment>
        <rdfs:label xml:lang="en">has lattice point</rdfs:label>
    </owl:ObjectProperty>
    


    <!-- https://purls.helmholtz-metadaten.de/disos/diso#hasLineSense -->

    <owl:ObjectProperty rdf:about="https://purls.helmholtz-metadaten.de/disos/diso#hasLineSense">
        <rdfs:domain rdf:resource="https://purls.helmholtz-metadaten.de/disos/diso#Dislocation"/>
        <rdfs:range rdf:resource="https://purls.helmholtz-metadaten.de/disos/diso#LineSense"/>
        <rdfs:comment xml:lang="en">hasLineSense represents the relationship between dislocation and line sense.</rdfs:comment>
        <rdfs:label xml:lang="en">has line sense</rdfs:label>
    </owl:ObjectProperty>
    


    <!-- https://purls.helmholtz-metadaten.de/disos/diso#hasMathematicalRepresentation -->

    <owl:ObjectProperty rdf:about="https://purls.helmholtz-metadaten.de/disos/diso#hasMathematicalRepresentation">
        <rdfs:subPropertyOf rdf:resource="https://purls.helmholtz-metadaten.de/disos/diso#hasRepresentation"/>
        <rdfs:domain rdf:resource="https://purls.helmholtz-metadaten.de/disos/diso#Dislocation"/>
        <rdfs:range rdf:resource="https://purls.helmholtz-metadaten.de/disos/diso#Line"/>
        <rdfs:comment xml:lang="en">hasMathematicalRepresentation relates the entity with its mathematical representation.</rdfs:comment>
        <rdfs:label xml:lang="en">has mathematical representation</rdfs:label>
    </owl:ObjectProperty>
    


    <!-- https://purls.helmholtz-metadaten.de/disos/diso#hasNode -->

    <owl:ObjectProperty rdf:about="https://purls.helmholtz-metadaten.de/disos/diso#hasNode">
        <rdfs:domain rdf:resource="https://purls.helmholtz-metadaten.de/disos/diso#Segment"/>
        <rdfs:range rdf:resource="https://purls.helmholtz-metadaten.de/disos/diso#Node"/>
        <rdfs:comment xml:lang="en">hasNode represents the relationship between segment and node.</rdfs:comment>
        <rdfs:label xml:lang="en">has node</rdfs:label>
    </owl:ObjectProperty>
    


    <!-- https://purls.helmholtz-metadaten.de/disos/diso#hasNumericalRepresentation -->

    <owl:ObjectProperty rdf:about="https://purls.helmholtz-metadaten.de/disos/diso#hasNumericalRepresentation">
        <rdfs:subPropertyOf rdf:resource="https://purls.helmholtz-metadaten.de/disos/diso#hasRepresentation"/>
        <rdfs:domain rdf:resource="https://purls.helmholtz-metadaten.de/disos/diso#Line"/>
        <rdfs:range rdf:resource="https://purls.helmholtz-metadaten.de/disos/diso#DiscretizedLine"/>
        <rdfs:comment xml:lang="en">hasNumericalRepresentation relates the entity with its numerical representation.</rdfs:comment>
        <rdfs:label xml:lang="en">has numerical representation</rdfs:label>
    </owl:ObjectProperty>
    


    <!-- https://purls.helmholtz-metadaten.de/disos/diso#hasOutputDislocationStructure -->

    <owl:ObjectProperty rdf:about="https://purls.helmholtz-metadaten.de/disos/diso#hasOutputDislocationStructure">
        <rdfs:subPropertyOf rdf:resource="https://w3id.org/mdo/core/hasOutputStructure"/>
        <rdfs:domain rdf:resource="https://purls.helmholtz-metadaten.de/disos/diso#DDDSimulation"/>
        <rdfs:range rdf:resource="https://purls.helmholtz-metadaten.de/disos/diso#DislocationStructure"/>
        <rdfs:label xml:lang="en">has output dislocation structure</rdfs:label>
    </owl:ObjectProperty>
    


    <!-- https://purls.helmholtz-metadaten.de/disos/diso#hasRepresentation -->

    <owl:ObjectProperty rdf:about="https://purls.helmholtz-metadaten.de/disos/diso#hasRepresentation">
        <rdfs:domain rdf:resource="http://www.w3.org/2002/07/owl#Thing"/>
        <rdfs:range>
            <owl:Class>
                <owl:unionOf rdf:parseType="Collection">
                    <rdf:Description rdf:about="https://purls.helmholtz-metadaten.de/disos/diso#DiscretizedLine"/>
                    <rdf:Description rdf:about="https://purls.helmholtz-metadaten.de/disos/diso#Line"/>
                </owl:unionOf>
            </owl:Class>
        </rdfs:range>
        <rdfs:comment xml:lang="en">hasRepresentation relates the entity to another representation of entity.</rdfs:comment>
        <rdfs:label xml:lang="en">has representation</rdfs:label>
    </owl:ObjectProperty>
    


    <!-- https://purls.helmholtz-metadaten.de/disos/diso#hasSegment -->

    <owl:ObjectProperty rdf:about="https://purls.helmholtz-metadaten.de/disos/diso#hasSegment">
        <owl:inverseOf rdf:resource="https://purls.helmholtz-metadaten.de/disos/diso#isSegmentOf"/>
        <rdfs:domain rdf:resource="https://purls.helmholtz-metadaten.de/disos/diso#DiscretizedLine"/>
        <rdfs:range rdf:resource="https://purls.helmholtz-metadaten.de/disos/diso#Segment"/>
        <rdfs:comment xml:lang="en">hasSegment represents the relationship between discretized line and segment.</rdfs:comment>
        <rdfs:label xml:lang="en">has segment</rdfs:label>
    </owl:ObjectProperty>
    


    <!-- https://purls.helmholtz-metadaten.de/disos/diso#hasShapeFunction -->

    <owl:ObjectProperty rdf:about="https://purls.helmholtz-metadaten.de/disos/diso#hasShapeFunction">
        <rdfs:domain rdf:resource="https://purls.helmholtz-metadaten.de/disos/diso#DiscretizedLine"/>
        <rdfs:range rdf:resource="https://purls.helmholtz-metadaten.de/disos/diso#ShapeFunction"/>
        <rdfs:comment xml:lang="en">hasShapeFunction represents the relationship between discretized line and shape function.</rdfs:comment>
        <rdfs:label xml:lang="en">has shape function</rdfs:label>
    </owl:ObjectProperty>
    


    <!-- https://purls.helmholtz-metadaten.de/disos/diso#hasSlipDirection -->

    <owl:ObjectProperty rdf:about="https://purls.helmholtz-metadaten.de/disos/diso#hasSlipDirection">
        <rdfs:subPropertyOf rdf:resource="https://purls.helmholtz-metadaten.de/disos/diso#hasLatticeDirection"/>
        <rdfs:domain>
            <owl:Class>
                <owl:unionOf rdf:parseType="Collection">
                    <rdf:Description rdf:about="https://purls.helmholtz-metadaten.de/disos/diso#SlipPlane"/>
                    <rdf:Description rdf:about="https://purls.helmholtz-metadaten.de/disos/diso#SlipSystem"/>
                </owl:unionOf>
            </owl:Class>
        </rdfs:domain>
        <rdfs:range rdf:resource="https://purls.helmholtz-metadaten.de/disos/diso#SlipDirection"/>
        <rdfs:comment xml:lang="en">hasSlipDirection represents the relationship between the slip plane or slip system with the slip direction.</rdfs:comment>
        <rdfs:label xml:lang="en">has slip direction</rdfs:label>
    </owl:ObjectProperty>
    


    <!-- https://purls.helmholtz-metadaten.de/disos/diso#hasSlipPlane -->

    <owl:ObjectProperty rdf:about="https://purls.helmholtz-metadaten.de/disos/diso#hasSlipPlane">
        <rdfs:subPropertyOf rdf:resource="https://purls.helmholtz-metadaten.de/disos/diso#hasLatticePlane"/>
        <rdfs:domain rdf:resource="https://purls.helmholtz-metadaten.de/disos/cso#CrystalStructure"/>
        <rdfs:range rdf:resource="https://purls.helmholtz-metadaten.de/disos/diso#SlipPlane"/>
        <rdfs:comment xml:lang="en">hasSlipPlane represents the relationship between crystal structure and slip plane.</rdfs:comment>
        <rdfs:label xml:lang="en">has slip plane</rdfs:label>
    </owl:ObjectProperty>
    


    <!-- https://purls.helmholtz-metadaten.de/disos/diso#hasSlipPlaneNormal -->

    <owl:ObjectProperty rdf:about="https://purls.helmholtz-metadaten.de/disos/diso#hasSlipPlaneNormal">
        <rdfs:domain>
            <owl:Class>
                <owl:unionOf rdf:parseType="Collection">
                    <rdf:Description rdf:about="https://purls.helmholtz-metadaten.de/disos/diso#SlipPlane"/>
                    <rdf:Description rdf:about="https://purls.helmholtz-metadaten.de/disos/diso#SlipSystem"/>
                </owl:unionOf>
            </owl:Class>
        </rdfs:domain>
        <rdfs:range rdf:resource="https://purls.helmholtz-metadaten.de/disos/diso#SlipPlaneNormal"/>
        <rdfs:comment xml:lang="en">hasSlipPlaneNormal represents the relationship between a slip plane or slip system with slip plane normal.</rdfs:comment>
        <rdfs:label xml:lang="en">has slip plane normal</rdfs:label>
    </owl:ObjectProperty>
    


    <!-- https://purls.helmholtz-metadaten.de/disos/diso#hasSlipSystem -->

    <owl:ObjectProperty rdf:about="https://purls.helmholtz-metadaten.de/disos/diso#hasSlipSystem">
        <rdfs:domain rdf:resource="https://purls.helmholtz-metadaten.de/disos/cso#CrystalStructure"/>
        <rdfs:range rdf:resource="https://purls.helmholtz-metadaten.de/disos/diso#SlipSystem"/>
        <rdfs:comment xml:lang="en">hasSlipSystem represents the relationship between a crystal structure and slip system.</rdfs:comment>
        <rdfs:label xml:lang="en">has slip system</rdfs:label>
    </owl:ObjectProperty>
    


    <!-- https://purls.helmholtz-metadaten.de/disos/diso#hasStartNode -->

    <owl:ObjectProperty rdf:about="https://purls.helmholtz-metadaten.de/disos/diso#hasStartNode">
        <rdfs:subPropertyOf rdf:resource="https://purls.helmholtz-metadaten.de/disos/diso#hasNode"/>
        <rdfs:domain rdf:resource="https://purls.helmholtz-metadaten.de/disos/diso#Segment"/>
        <rdfs:range rdf:resource="https://purls.helmholtz-metadaten.de/disos/diso#Node"/>
        <rdfs:comment xml:lang="en">Sub-property of hasNode that relates the segment with the start node.</rdfs:comment>
        <rdfs:label xml:lang="en">has start node</rdfs:label>
    </owl:ObjectProperty>
    


    <!-- https://purls.helmholtz-metadaten.de/disos/diso#hasVectorOrigin -->

    <owl:ObjectProperty rdf:about="https://purls.helmholtz-metadaten.de/disos/diso#hasVectorOrigin">
        <rdfs:domain rdf:resource="https://purls.helmholtz-metadaten.de/disos/diso#LatticePlane"/>
        <rdfs:range rdf:resource="https://purls.helmholtz-metadaten.de/disos/diso#VectorOrigin"/>
        <rdfs:comment xml:lang="en">hasVectorOrigin represents the relationship between lattice plane and origin.</rdfs:comment>
        <rdfs:label xml:lang="en">has vector origin</rdfs:label>
    </owl:ObjectProperty>
    


    <!-- https://purls.helmholtz-metadaten.de/disos/diso#isSegmentOf -->

    <owl:ObjectProperty rdf:about="https://purls.helmholtz-metadaten.de/disos/diso#isSegmentOf">
        <rdfs:domain rdf:resource="https://purls.helmholtz-metadaten.de/disos/diso#Segment"/>
        <rdfs:range rdf:resource="https://purls.helmholtz-metadaten.de/disos/diso#DiscretizedLine"/>
        <rdfs:comment xml:lang="en">Inverse of hasSegment</rdfs:comment>
        <rdfs:label xml:lang="en">is segment of</rdfs:label>
    </owl:ObjectProperty>
    


    <!-- https://purls.helmholtz-metadaten.de/disos/diso#movesOn -->

    <owl:ObjectProperty rdf:about="https://purls.helmholtz-metadaten.de/disos/diso#movesOn">
        <rdfs:domain rdf:resource="https://purls.helmholtz-metadaten.de/disos/diso#Dislocation"/>
        <rdfs:range rdf:resource="https://purls.helmholtz-metadaten.de/disos/diso#SlipPlane"/>
        <rdfs:comment xml:lang="en">movesOn represents the relationship between dislocation and slip plane.</rdfs:comment>
        <rdfs:label xml:lang="en">moves on</rdfs:label>
    </owl:ObjectProperty>
    


    <!-- https://purls.helmholtz-metadaten.de/disos/diso#observedBy -->

    <owl:ObjectProperty rdf:about="https://purls.helmholtz-metadaten.de/disos/diso#observedBy">
        <rdfs:domain rdf:resource="https://purls.helmholtz-metadaten.de/disos/diso#Dislocation"/>
        <rdfs:range>
            <owl:Class>
                <owl:unionOf rdf:parseType="Collection">
                    <rdf:Description rdf:about="https://purls.helmholtz-metadaten.de/disos/diso#FieldIonMicroscopy"/>
                    <rdf:Description rdf:about="https://purls.helmholtz-metadaten.de/disos/diso#TransmissionElectronMicroscopy"/>
                </owl:unionOf>
            </owl:Class>
        </rdfs:range>
        <rdfs:comment xml:lang="en">observedBy represents the relationship between dislocation and microscopy techniques, e.g., TEM, FIM, etc.</rdfs:comment>
        <rdfs:label xml:lang="en">observed by</rdfs:label>
    </owl:ObjectProperty>
    


    <!-- https://purls.helmholtz-metadaten.de/disos/diso#relatesToCrystallineMaterial -->

    <owl:ObjectProperty rdf:about="https://purls.helmholtz-metadaten.de/disos/diso#relatesToCrystallineMaterial">
        <rdfs:label xml:lang="en">relates to crystalline material</rdfs:label>
    </owl:ObjectProperty>
    


    <!-- https://purls.helmholtz-metadaten.de/disos/diso#resultsIn -->

    <owl:ObjectProperty rdf:about="https://purls.helmholtz-metadaten.de/disos/diso#resultsIn">
        <rdfs:domain rdf:resource="https://purls.helmholtz-metadaten.de/disos/diso#Dislocation"/>
        <rdfs:range rdf:resource="https://purls.helmholtz-metadaten.de/disos/diso#LatticeDisplacement"/>
        <rdfs:comment xml:lang="en">resultsIn represents the relationship between dislocation and lattice displacement.</rdfs:comment>
        <rdfs:label xml:lang="en">results in</rdfs:label>
    </owl:ObjectProperty>
    


    <!-- 
    ///////////////////////////////////////////////////////////////////////////////////////
    //
    // Data properties
    //
    ///////////////////////////////////////////////////////////////////////////////////////
     -->

    


    <!-- http://purls.helmholtz-metadaten.de/mwo/hasORCID -->

    <owl:DatatypeProperty rdf:about="http://purls.helmholtz-metadaten.de/mwo/hasORCID"/>
    


    <!-- http://www.w3.org/ns/prov#endedAtTime -->

    <owl:DatatypeProperty rdf:about="http://www.w3.org/ns/prov#endedAtTime"/>
    


    <!-- http://www.w3.org/ns/prov#startedAtTime -->

    <owl:DatatypeProperty rdf:about="http://www.w3.org/ns/prov#startedAtTime"/>
    


    <!-- http://xmlns.com/foaf/0.1/family_name -->

    <owl:DatatypeProperty rdf:about="http://xmlns.com/foaf/0.1/family_name"/>
    


    <!-- http://xmlns.com/foaf/0.1/firstName -->

    <owl:DatatypeProperty rdf:about="http://xmlns.com/foaf/0.1/firstName"/>
    


    <!-- https://purls.helmholtz-metadaten.de/disos/cso#firstAxisComponent -->

    <owl:DatatypeProperty rdf:about="https://purls.helmholtz-metadaten.de/disos/cso#firstAxisComponent"/>
    


    <!-- https://purls.helmholtz-metadaten.de/disos/cso#secondAxisComponent -->

    <owl:DatatypeProperty rdf:about="https://purls.helmholtz-metadaten.de/disos/cso#secondAxisComponent"/>
    


    <!-- https://purls.helmholtz-metadaten.de/disos/cso#thirdAxisComponent -->

    <owl:DatatypeProperty rdf:about="https://purls.helmholtz-metadaten.de/disos/cso#thirdAxisComponent"/>
    


    <!-- https://purls.helmholtz-metadaten.de/disos/cso#vectorMagnitude -->

    <owl:DatatypeProperty rdf:about="https://purls.helmholtz-metadaten.de/disos/cso#vectorMagnitude"/>
    


    <!-- https://purls.helmholtz-metadaten.de/disos/diso#directionMillerIndice -->

    <owl:DatatypeProperty rdf:about="https://purls.helmholtz-metadaten.de/disos/diso#directionMillerIndice">
        <rdfs:domain>
            <owl:Class>
                <owl:unionOf rdf:parseType="Collection">
                    <rdf:Description rdf:about="https://purls.helmholtz-metadaten.de/disos/diso#LatticeDirection"/>
                    <rdf:Description rdf:about="https://purls.helmholtz-metadaten.de/disos/diso#SlipPlaneNormal"/>
                </owl:unionOf>
            </owl:Class>
        </rdfs:domain>
        <rdfs:range rdf:resource="http://www.w3.org/2001/XMLSchema#string"/>
        <rdfs:comment xml:lang="en">directionMillerIndice represents Miller indice of lattice direction in string.</rdfs:comment>
        <rdfs:label xml:lang="en">direction miller indice</rdfs:label>
    </owl:DatatypeProperty>
    


    <!-- https://purls.helmholtz-metadaten.de/disos/diso#familyDirectionMillerIndice -->

    <owl:DatatypeProperty rdf:about="https://purls.helmholtz-metadaten.de/disos/diso#familyDirectionMillerIndice">
        <rdfs:domain rdf:resource="https://purls.helmholtz-metadaten.de/disos/diso#FamilyOfCrystalDirection"/>
        <rdfs:range rdf:resource="http://www.w3.org/2001/XMLSchema#string"/>
        <rdfs:comment xml:lang="en">familyDirectionMillerIndice represents a set of miller indices of lattice direction in string.</rdfs:comment>
        <rdfs:label xml:lang="en">family direction miller indice</rdfs:label>
    </owl:DatatypeProperty>
    


    <!-- https://purls.helmholtz-metadaten.de/disos/diso#familyPlaneMillerIndice -->

    <owl:DatatypeProperty rdf:about="https://purls.helmholtz-metadaten.de/disos/diso#familyPlaneMillerIndice">
        <rdfs:domain rdf:resource="https://purls.helmholtz-metadaten.de/disos/diso#FamilyOfCrystalPlane"/>
        <rdfs:range rdf:resource="http://www.w3.org/2001/XMLSchema#string"/>
        <rdfs:comment xml:lang="en">familyPlaneMillerIndice represents a set of Miller indice of lattice plane in string.</rdfs:comment>
        <rdfs:label xml:lang="en">family plane miller indice</rdfs:label>
    </owl:DatatypeProperty>
    


    <!-- https://purls.helmholtz-metadaten.de/disos/diso#planeMillerIndice -->

    <owl:DatatypeProperty rdf:about="https://purls.helmholtz-metadaten.de/disos/diso#planeMillerIndice">
        <rdfs:domain rdf:resource="https://purls.helmholtz-metadaten.de/disos/diso#LatticePlane"/>
        <rdfs:range rdf:resource="http://www.w3.org/2001/XMLSchema#string"/>
        <rdfs:comment xml:lang="en">planeMillerIndice represents Miller indice of lattice plane in string.</rdfs:comment>
        <rdfs:label xml:lang="en">plane miller indice</rdfs:label>
    </owl:DatatypeProperty>
    


    <!-- https://purls.helmholtz-metadaten.de/disos/diso#slipArea -->

    <owl:DatatypeProperty rdf:about="https://purls.helmholtz-metadaten.de/disos/diso#slipArea">
        <rdfs:domain rdf:resource="https://purls.helmholtz-metadaten.de/disos/diso#DiscretizedLine"/>
        <rdfs:range rdf:resource="http://www.w3.org/2001/XMLSchema#double"/>
        <rdfs:comment xml:lang="en">slipArea represents the slip area of discretized line in double.</rdfs:comment>
        <rdfs:label xml:lang="en">slipArea</rdfs:label>
    </owl:DatatypeProperty>
    


    <!-- https://purls.helmholtz-metadaten.de/disos/diso#softwareVersion -->

    <owl:DatatypeProperty rdf:about="https://purls.helmholtz-metadaten.de/disos/diso#softwareVersion">
        <rdfs:label xml:lang="en">software version</rdfs:label>
    </owl:DatatypeProperty>
    


    <!-- https://w3id.org/mdo/provenance/SoftwareName -->

    <owl:DatatypeProperty rdf:about="https://w3id.org/mdo/provenance/SoftwareName">
        <rdfs:label xml:lang="en">software name</rdfs:label>
    </owl:DatatypeProperty>
    


    <!-- https://w3id.org/mdo/structure/X_axisCoordinate -->

    <owl:DatatypeProperty rdf:about="https://w3id.org/mdo/structure/X_axisCoordinate"/>
    


    <!-- https://w3id.org/mdo/structure/Y_axisCoordinate -->

    <owl:DatatypeProperty rdf:about="https://w3id.org/mdo/structure/Y_axisCoordinate"/>
    


    <!-- https://w3id.org/mdo/structure/Z_axisCoordinate -->

    <owl:DatatypeProperty rdf:about="https://w3id.org/mdo/structure/Z_axisCoordinate"/>
    


    <!-- 
    ///////////////////////////////////////////////////////////////////////////////////////
    //
    // Classes
    //
    ///////////////////////////////////////////////////////////////////////////////////////
     -->

    


    <!-- http://emmo.info/domain-crystallography/crystallography#EMMO_69dab453_6596_464d_a21d_d64643f4ed9b -->

    <owl:Class rdf:about="http://emmo.info/domain-crystallography/crystallography#EMMO_69dab453_6596_464d_a21d_d64643f4ed9b">
        <owl:equivalentClass rdf:resource="https://purls.helmholtz-metadaten.de/disos/cdo#CrystallineMaterial"/>
        <rdfs:subClassOf rdf:resource="http://emmo.info/emmo#EMMO_a2b006f2_bbfd_4dba_bcaa_3fca20cd6be1"/>
        <skos:prefLabel xml:lang="en">Crystal</skos:prefLabel>
    </owl:Class>
    


    <!-- http://emmo.info/domain-crystallography/crystallography#EMMO_6a340d67_c6cb_4348_8537_d9aa0e768721 -->

    <owl:Class rdf:about="http://emmo.info/domain-crystallography/crystallography#EMMO_6a340d67_c6cb_4348_8537_d9aa0e768721">
        <owl:equivalentClass rdf:resource="https://purls.helmholtz-metadaten.de/disos/cso#CrystalStructure"/>
        <rdfs:subClassOf rdf:resource="http://emmo.info/domain-crystallography/crystallography#EMMO_78a3d6f9_0bbd_4b44_a9a9_baf3df276a06"/>
        <rdfs:subClassOf>
            <owl:Restriction>
                <owl:onProperty>
                    <rdf:Description>
                        <owl:inverseOf rdf:resource="http://emmo.info/emmo#EMMO_e1097637_70d2_4895_973f_2396f04fa204"/>
                    </rdf:Description>
                </owl:onProperty>
                <owl:someValuesFrom rdf:resource="http://emmo.info/domain-crystallography/crystallography#EMMO_69dab453_6596_464d_a21d_d64643f4ed9b"/>
            </owl:Restriction>
        </rdfs:subClassOf>
        <skos:prefLabel xml:lang="en">CrystalStructure</skos:prefLabel>
    </owl:Class>
    


    <!-- http://emmo.info/domain-crystallography/crystallography#EMMO_78a3d6f9_0bbd_4b44_a9a9_baf3df276a06 -->

    <owl:Class rdf:about="http://emmo.info/domain-crystallography/crystallography#EMMO_78a3d6f9_0bbd_4b44_a9a9_baf3df276a06">
        <rdfs:subClassOf rdf:resource="http://emmo.info/emmo#EMMO_d8d2144e_5c8d_455d_a643_5caf4d8d9df8"/>
        <skos:prefLabel xml:lang="en">Crystallographical</skos:prefLabel>
    </owl:Class>
    


    <!-- http://emmo.info/emmo#EMMO_4ce76d7f_03f8_45b6_9003_90052a79bfaa -->

    <owl:Class rdf:about="http://emmo.info/emmo#EMMO_4ce76d7f_03f8_45b6_9003_90052a79bfaa">
        <rdfs:subClassOf rdf:resource="http://emmo.info/emmo#EMMO_54ee6b5e_5261_44a8_86eb_5717e7fdb9d0"/>
        <skos:prefLabel xml:lang="en">Numerical</skos:prefLabel>
    </owl:Class>
    


    <!-- http://emmo.info/emmo#EMMO_54ee6b5e_5261_44a8_86eb_5717e7fdb9d0 -->

    <owl:Class rdf:about="http://emmo.info/emmo#EMMO_54ee6b5e_5261_44a8_86eb_5717e7fdb9d0">
        <rdfs:subClassOf rdf:resource="http://emmo.info/emmo#EMMO_d8d2144e_5c8d_455d_a643_5caf4d8d9df8"/>
        <skos:prefLabel xml:lang="en">Mathematical</skos:prefLabel>
    </owl:Class>
    


    <!-- http://emmo.info/emmo#EMMO_a2b006f2_bbfd_4dba_bcaa_3fca20cd6be1 -->

    <owl:Class rdf:about="http://emmo.info/emmo#EMMO_a2b006f2_bbfd_4dba_bcaa_3fca20cd6be1">
        <skos:prefLabel xml:lang="en">Solid</skos:prefLabel>
    </owl:Class>
    


    <!-- http://emmo.info/emmo#EMMO_d8d2144e_5c8d_455d_a643_5caf4d8d9df8 -->

    <owl:Class rdf:about="http://emmo.info/emmo#EMMO_d8d2144e_5c8d_455d_a643_5caf4d8d9df8">
        <skos:prefLabel xml:lang="en">Language</skos:prefLabel>
    </owl:Class>
    


    <!-- http://emmo.info/emmo#EMMO_f7ed665b_c2e1_42bc_889b_6b42ed3a36f0 -->

    <owl:Class rdf:about="http://emmo.info/emmo#EMMO_f7ed665b_c2e1_42bc_889b_6b42ed3a36f0">
        <rdfs:subClassOf rdf:resource="http://emmo.info/emmo#EMMO_54ee6b5e_5261_44a8_86eb_5717e7fdb9d0"/>
        <skos:prefLabel xml:lang="en">MathematicalModel</skos:prefLabel>
    </owl:Class>
    


    <!-- http://qudt.org/schema/qudt/Quantity -->

    <owl:Class rdf:about="http://qudt.org/schema/qudt/Quantity">
        <rdfs:subClassOf>
            <owl:Restriction>
                <owl:onProperty rdf:resource="http://qudt.org/schema/qudt/hasQuantityKind"/>
                <owl:allValuesFrom rdf:resource="http://qudt.org/schema/qudt/QuantityKind"/>
            </owl:Restriction>
        </rdfs:subClassOf>
        <rdfs:subClassOf>
            <owl:Restriction>
                <owl:onProperty rdf:resource="http://qudt.org/schema/qudt/quantityValue"/>
                <owl:allValuesFrom rdf:resource="http://qudt.org/schema/qudt/QuantityValue"/>
            </owl:Restriction>
        </rdfs:subClassOf>
        <qudt:description rdf:datatype="http://www.w3.org/1999/02/22-rdf-syntax-ns#HTML">&lt;p class=&quot;lm-para&quot;&gt;A quantity is the measurement of an observable property of a particular object, event, or physical system. A quantity is always associated with the context of measurement (i.e. the thing measured, the measured value, the accuracy of measurement, etc.) whereas the underlying quantity kind is independent of any particular measurement. Thus, length is a quantity kind while the height of a rocket is a specific quantity of length; its magnitude that may be expressed in meters, feet, inches, etc. Examples of physical quantities include physical constants, such as the speed of light in a vacuum, Planck&apos;s constant, the electric permittivity of free space, and the fine structure constant. &lt;/p&gt;

&lt;p class=&quot;lm-para&quot;&gt;In other words, quantities are quantifiable aspects of the world, such as time, distance, velocity, mass, momentum, energy, and weight, and units are used to describe their measure. Many of which are related to each other by various physical laws, and as a result the units of some of the quantities can be expressed as products (or ratios) of powers of other units (e.g., momentum is mass times velocity and velocity is measured in distance divided by time). These relationships are discussed in dimensional analysis. Those that cannot be so expressed can be regarded as &quot;fundamental&quot; in this sense.&lt;/p&gt;
&lt;p class=&quot;lm-para&quot;&gt;A quantity is distinguished from a &quot;quantity kind&quot; in that the former carries a value and the latter is a type specifier.&lt;/p&gt;</qudt:description>
        <rdfs:isDefinedBy rdf:resource="http://qudt.org/2.0/schema/qudt"/>
        <rdfs:isDefinedBy rdf:resource="http://qudt.org/schema/qudt"/>
        <rdfs:label>Quantity</rdfs:label>
    </owl:Class>
    


    <!-- http://qudt.org/schema/qudt/QuantityKind -->

    <owl:Class rdf:about="http://qudt.org/schema/qudt/QuantityKind">
        <qudt:description rdf:datatype="http://www.w3.org/1999/02/22-rdf-syntax-ns#HTML">A &lt;b&gt;Quantity Kind&lt;/b&gt; is any observable property that can be  measured and quantified numerically. Familiar examples include physical properties such as length, mass, time, force, energy, power, electric charge, etc. Less familiar examples include currency, interest rate, price to earning ratio, and information capacity.</qudt:description>
        <rdfs:isDefinedBy rdf:resource="http://qudt.org/2.0/schema/qudt"/>
        <rdfs:isDefinedBy rdf:resource="http://qudt.org/schema/qudt"/>
        <rdfs:label>Quantity Kind</rdfs:label>
    </owl:Class>
    


    <!-- http://qudt.org/schema/qudt/QuantityValue -->

    <owl:Class rdf:about="http://qudt.org/schema/qudt/QuantityValue">
        <rdfs:subClassOf>
            <owl:Restriction>
                <owl:onProperty rdf:resource="http://qudt.org/schema/qudt/unit"/>
                <owl:allValuesFrom rdf:resource="http://qudt.org/schema/qudt/Unit"/>
            </owl:Restriction>
        </rdfs:subClassOf>
        <qudt:description rdf:datatype="http://www.w3.org/1999/02/22-rdf-syntax-ns#HTML">A &lt;i&gt;Quantity Value&lt;/i&gt; expresses the magnitude and kind of a quantity and is given by the product of a numerical value &lt;code&gt;n&lt;/code&gt; and a unit of measure &lt;code&gt;U&lt;/code&gt;. The number multiplying the unit is referred to as the numerical value of the quantity expressed in that unit. Refer to &lt;a href=&quot;http://physics.nist.gov/Pubs/SP811/sec07.html&quot;&gt;NIST SP 811 section 7&lt;/a&gt; for more on quantity values.</qudt:description>
        <rdfs:isDefinedBy rdf:resource="http://qudt.org/2.0/schema/qudt"/>
        <rdfs:isDefinedBy rdf:resource="http://qudt.org/schema/qudt"/>
        <rdfs:label>Quantity value</rdfs:label>
    </owl:Class>
    


    <!-- http://qudt.org/schema/qudt/Unit -->

    <owl:Class rdf:about="http://qudt.org/schema/qudt/Unit">
        <qudt:description rdf:datatype="http://www.w3.org/1999/02/22-rdf-syntax-ns#HTML">A unit of measure, or unit, is a particular quantity value that has been chosen as a scale for measuring other quantities the same kind (more generally of equivalent dimension). For example, the meter is a quantity of length that has been rigorously defined and standardized by the BIPM (International Board of Weights and Measures). Any measurement of the length can be expressed as a number multiplied by the unit meter. More formally, the value of a physical quantity Q with respect to a unit (U) is expressed as the scalar multiple of a real number (n) and U, as  \(Q = nU\).</qudt:description>
        <rdfs:isDefinedBy rdf:resource="http://qudt.org/2.0/schema/qudt"/>
        <rdfs:isDefinedBy rdf:resource="http://qudt.org/schema/qudt"/>
        <rdfs:label>Unit</rdfs:label>
    </owl:Class>
    


    <!-- http://www.w3.org/ns/prov#Activity -->

    <owl:Class rdf:about="http://www.w3.org/ns/prov#Activity">
        <rdfs:subClassOf>
            <owl:Restriction>
                <owl:onProperty rdf:resource="http://www.w3.org/ns/prov#endedAtTime"/>
                <owl:someValuesFrom rdf:resource="http://www.w3.org/2001/XMLSchema#dateTime"/>
            </owl:Restriction>
        </rdfs:subClassOf>
        <rdfs:subClassOf>
            <owl:Restriction>
                <owl:onProperty rdf:resource="http://www.w3.org/ns/prov#startedAtTime"/>
                <owl:someValuesFrom rdf:resource="http://www.w3.org/2001/XMLSchema#dateTime"/>
            </owl:Restriction>
        </rdfs:subClassOf>
    </owl:Class>
    


    <!-- http://www.w3.org/ns/prov#Agent -->

    <owl:Class rdf:about="http://www.w3.org/ns/prov#Agent"/>
    


    <!-- http://www.w3.org/ns/prov#Person -->

    <owl:Class rdf:about="http://www.w3.org/ns/prov#Person">
        <rdfs:subClassOf rdf:resource="http://www.w3.org/ns/prov#Agent"/>
        <rdfs:subClassOf>
            <owl:Restriction>
                <owl:onProperty rdf:resource="http://purls.helmholtz-metadaten.de/mwo/hasORCID"/>
                <owl:someValuesFrom rdf:resource="http://www.w3.org/2001/XMLSchema#string"/>
            </owl:Restriction>
        </rdfs:subClassOf>
        <rdfs:subClassOf>
            <owl:Restriction>
                <owl:onProperty rdf:resource="http://xmlns.com/foaf/0.1/family_name"/>
                <owl:someValuesFrom rdf:resource="http://www.w3.org/2001/XMLSchema#string"/>
            </owl:Restriction>
        </rdfs:subClassOf>
        <rdfs:subClassOf>
            <owl:Restriction>
                <owl:onProperty rdf:resource="http://xmlns.com/foaf/0.1/firstName"/>
                <owl:someValuesFrom rdf:resource="http://www.w3.org/2001/XMLSchema#string"/>
            </owl:Restriction>
        </rdfs:subClassOf>
    </owl:Class>
    


    <!-- http://www.w3.org/ns/prov#SoftwareAgent -->

    <owl:Class rdf:about="http://www.w3.org/ns/prov#SoftwareAgent">
        <rdfs:subClassOf rdf:resource="http://www.w3.org/ns/prov#Agent"/>
        <rdfs:subClassOf>
            <owl:Restriction>
                <owl:onProperty rdf:resource="https://purls.helmholtz-metadaten.de/disos/diso#softwareVersion"/>
                <owl:someValuesFrom rdf:resource="http://www.w3.org/2001/XMLSchema#string"/>
            </owl:Restriction>
        </rdfs:subClassOf>
        <rdfs:subClassOf>
            <owl:Restriction>
                <owl:onProperty rdf:resource="https://w3id.org/mdo/provenance/SoftwareName"/>
                <owl:someValuesFrom rdf:resource="http://www.w3.org/2001/XMLSchema#string"/>
            </owl:Restriction>
        </rdfs:subClassOf>
    </owl:Class>
    


    <!-- https://purls.helmholtz-metadaten.de/disos/cdo#CrystallineMaterial -->

    <owl:Class rdf:about="https://purls.helmholtz-metadaten.de/disos/cdo#CrystallineMaterial">
        <rdfs:subClassOf>
            <owl:Class>
                <owl:intersectionOf rdf:parseType="Collection">
                    <owl:Restriction>
                        <owl:onProperty rdf:resource="https://purls.helmholtz-metadaten.de/disos/cdo#hasCrystalStructure"/>
                        <owl:someValuesFrom rdf:resource="http://emmo.info/domain-crystallography/crystallography#EMMO_6a340d67_c6cb_4348_8537_d9aa0e768721"/>
                    </owl:Restriction>
                    <owl:Restriction>
                        <owl:onProperty rdf:resource="https://purls.helmholtz-metadaten.de/disos/cdo#hasCrystalStructure"/>
                        <owl:allValuesFrom rdf:resource="http://emmo.info/domain-crystallography/crystallography#EMMO_6a340d67_c6cb_4348_8537_d9aa0e768721"/>
                    </owl:Restriction>
                </owl:intersectionOf>
            </owl:Class>
        </rdfs:subClassOf>
        <rdfs:subClassOf>
            <owl:Class>
                <owl:intersectionOf rdf:parseType="Collection">
                    <owl:Restriction>
                        <owl:onProperty rdf:resource="https://purls.helmholtz-metadaten.de/disos/cdo#hasCrystallographicDefect"/>
                        <owl:someValuesFrom rdf:resource="https://purls.helmholtz-metadaten.de/disos/cdo#CrystallographicDefect"/>
                    </owl:Restriction>
                    <owl:Restriction>
                        <owl:onProperty rdf:resource="https://purls.helmholtz-metadaten.de/disos/cdo#hasCrystallographicDefect"/>
                        <owl:allValuesFrom rdf:resource="https://purls.helmholtz-metadaten.de/disos/cdo#CrystallographicDefect"/>
                    </owl:Restriction>
                </owl:intersectionOf>
            </owl:Class>
        </rdfs:subClassOf>
        <rdfs:label xml:lang="en">Crystalline Material</rdfs:label>
    </owl:Class>
    


    <!-- https://purls.helmholtz-metadaten.de/disos/cdo#CrystallographicDefect -->

    <owl:Class rdf:about="https://purls.helmholtz-metadaten.de/disos/cdo#CrystallographicDefect">
        <rdfs:subClassOf rdf:resource="http://emmo.info/domain-crystallography/crystallography#EMMO_78a3d6f9_0bbd_4b44_a9a9_baf3df276a06"/>
        <rdfs:subClassOf>
            <owl:Restriction>
                <owl:onProperty>
                    <rdf:Description>
                        <owl:inverseOf rdf:resource="http://emmo.info/emmo#EMMO_e1097637_70d2_4895_973f_2396f04fa204"/>
                    </rdf:Description>
                </owl:onProperty>
                <owl:someValuesFrom rdf:resource="http://emmo.info/domain-crystallography/crystallography#EMMO_69dab453_6596_464d_a21d_d64643f4ed9b"/>
            </owl:Restriction>
        </rdfs:subClassOf>
        <rdfs:comment xml:lang="en">The crystallographic defect is a lattice irregularity that has one or more dimensions on the order of an atomic diameter.</rdfs:comment>
        <rdfs:label xml:lang="en">Crystallographic Defect</rdfs:label>
    </owl:Class>
    


    <!-- https://purls.helmholtz-metadaten.de/disos/cso#CrystalStructure -->

    <owl:Class rdf:about="https://purls.helmholtz-metadaten.de/disos/cso#CrystalStructure">
        <rdfs:subClassOf>
            <owl:Class>
                <owl:intersectionOf rdf:parseType="Collection">
                    <owl:Restriction>
                        <owl:onProperty rdf:resource="https://purls.helmholtz-metadaten.de/disos/diso#hasSlipPlane"/>
                        <owl:someValuesFrom rdf:resource="https://purls.helmholtz-metadaten.de/disos/diso#SlipPlane"/>
                    </owl:Restriction>
                    <owl:Restriction>
                        <owl:onProperty rdf:resource="https://purls.helmholtz-metadaten.de/disos/diso#hasSlipPlane"/>
                        <owl:allValuesFrom rdf:resource="https://purls.helmholtz-metadaten.de/disos/diso#SlipPlane"/>
                    </owl:Restriction>
                </owl:intersectionOf>
            </owl:Class>
        </rdfs:subClassOf>
        <rdfs:subClassOf>
            <owl:Class>
                <owl:intersectionOf rdf:parseType="Collection">
                    <owl:Restriction>
                        <owl:onProperty rdf:resource="https://purls.helmholtz-metadaten.de/disos/diso#hasSlipSystem"/>
                        <owl:someValuesFrom rdf:resource="https://purls.helmholtz-metadaten.de/disos/diso#SlipSystem"/>
                    </owl:Restriction>
                    <owl:Restriction>
                        <owl:onProperty rdf:resource="https://purls.helmholtz-metadaten.de/disos/diso#hasSlipSystem"/>
                        <owl:allValuesFrom rdf:resource="https://purls.helmholtz-metadaten.de/disos/diso#SlipSystem"/>
                    </owl:Restriction>
                </owl:intersectionOf>
            </owl:Class>
        </rdfs:subClassOf>
        <rdfs:comment xml:lang="en">A crystal structure is described by the lattice geometry and atomic arrangements within the unit cell.</rdfs:comment>
        <rdfs:label xml:lang="en">Crystal Structure</rdfs:label>
    </owl:Class>
    


    <!-- https://purls.helmholtz-metadaten.de/disos/cso#Lattice -->

    <owl:Class rdf:about="https://purls.helmholtz-metadaten.de/disos/cso#Lattice">
        <rdfs:subClassOf>
            <owl:Class>
                <owl:intersectionOf rdf:parseType="Collection">
                    <owl:Restriction>
                        <owl:onProperty rdf:resource="https://purls.helmholtz-metadaten.de/disos/diso#hasLatticeDirection"/>
                        <owl:someValuesFrom rdf:resource="https://purls.helmholtz-metadaten.de/disos/diso#LatticeDirection"/>
                    </owl:Restriction>
                    <owl:Restriction>
                        <owl:onProperty rdf:resource="https://purls.helmholtz-metadaten.de/disos/diso#hasLatticeDirection"/>
                        <owl:allValuesFrom rdf:resource="https://purls.helmholtz-metadaten.de/disos/diso#LatticeDirection"/>
                    </owl:Restriction>
                </owl:intersectionOf>
            </owl:Class>
        </rdfs:subClassOf>
        <rdfs:subClassOf>
            <owl:Class>
                <owl:intersectionOf rdf:parseType="Collection">
                    <owl:Restriction>
                        <owl:onProperty rdf:resource="https://purls.helmholtz-metadaten.de/disos/diso#hasLatticePlane"/>
                        <owl:someValuesFrom rdf:resource="https://purls.helmholtz-metadaten.de/disos/diso#LatticePlane"/>
                    </owl:Restriction>
                    <owl:Restriction>
                        <owl:onProperty rdf:resource="https://purls.helmholtz-metadaten.de/disos/diso#hasLatticeDirection"/>
                        <owl:allValuesFrom rdf:resource="https://purls.helmholtz-metadaten.de/disos/diso#LatticeDirection"/>
                    </owl:Restriction>
                </owl:intersectionOf>
            </owl:Class>
        </rdfs:subClassOf>
        <rdfs:subClassOf>
            <owl:Class>
                <owl:intersectionOf rdf:parseType="Collection">
                    <owl:Restriction>
                        <owl:onProperty rdf:resource="https://purls.helmholtz-metadaten.de/disos/diso#hasLatticePoint"/>
                        <owl:someValuesFrom rdf:resource="https://purls.helmholtz-metadaten.de/disos/diso#LatticePoint"/>
                    </owl:Restriction>
                    <owl:Restriction>
                        <owl:onProperty rdf:resource="https://purls.helmholtz-metadaten.de/disos/diso#hasLatticePoint"/>
                        <owl:allValuesFrom rdf:resource="https://purls.helmholtz-metadaten.de/disos/diso#LatticePoint"/>
                    </owl:Restriction>
                </owl:intersectionOf>
            </owl:Class>
        </rdfs:subClassOf>
        <rdfs:comment xml:lang="de">Das mathematische Konzept zur Darstellung der Periodizitt eines Kristalls. Ein Gitter definiert eine periodische Anordnung von einem oder mehreren Atomen.</rdfs:comment>
        <rdfs:comment xml:lang="en">The mathematical concept to represent the periodicity of a crystal. A lattice defines a periodic arrangement of one or more atoms.</rdfs:comment>
        <rdfs:label xml:lang="en">Lattice</rdfs:label>
    </owl:Class>
    


    <!-- https://purls.helmholtz-metadaten.de/disos/cso#Point -->

    <owl:Class rdf:about="https://purls.helmholtz-metadaten.de/disos/cso#Point">
        <rdfs:subClassOf>
            <owl:Restriction>
                <owl:onProperty rdf:resource="https://purls.helmholtz-metadaten.de/disos/cso#hasPositionVector"/>
                <owl:allValuesFrom rdf:resource="https://purls.helmholtz-metadaten.de/disos/cso#PositionVector"/>
            </owl:Restriction>
        </rdfs:subClassOf>
        <rdfs:comment xml:lang="en">In classical Euclidean geometry, a point is a primitive notion that models an exact location in the space, and has no length, width, or thickness.</rdfs:comment>
        <rdfs:label xml:lang="en">Point</rdfs:label>
    </owl:Class>
    


    <!-- https://purls.helmholtz-metadaten.de/disos/cso#PositionVector -->

    <owl:Class rdf:about="https://purls.helmholtz-metadaten.de/disos/cso#PositionVector">
        <rdfs:subClassOf rdf:resource="https://purls.helmholtz-metadaten.de/disos/cso#Vector"/>
        <rdfs:comment xml:lang="en">Euclidean vector that represents the position of a point P in space in relation to an arbitrary reference origin O.</rdfs:comment>
        <rdfs:label xml:lang="en">Position Vector</rdfs:label>
    </owl:Class>
    


    <!-- https://purls.helmholtz-metadaten.de/disos/cso#Vector -->

    <owl:Class rdf:about="https://purls.helmholtz-metadaten.de/disos/cso#Vector">
        <rdfs:subClassOf>
            <owl:Class>
                <owl:intersectionOf rdf:parseType="Collection">
                    <owl:Restriction>
                        <owl:onProperty rdf:resource="https://purls.helmholtz-metadaten.de/disos/cso#hasVectorComponent"/>
                        <owl:someValuesFrom rdf:resource="https://purls.helmholtz-metadaten.de/disos/cso#VectorComponentOfBasis"/>
                    </owl:Restriction>
                    <owl:Restriction>
                        <owl:onProperty rdf:resource="https://purls.helmholtz-metadaten.de/disos/cso#hasVectorComponent"/>
                        <owl:allValuesFrom rdf:resource="https://purls.helmholtz-metadaten.de/disos/cso#VectorComponentOfBasis"/>
                    </owl:Restriction>
                </owl:intersectionOf>
            </owl:Class>
        </rdfs:subClassOf>
        <rdfs:subClassOf>
            <owl:Restriction>
                <owl:onProperty rdf:resource="https://purls.helmholtz-metadaten.de/disos/cso#vectorMagnitude"/>
                <owl:qualifiedCardinality rdf:datatype="http://www.w3.org/2001/XMLSchema#nonNegativeInteger">1</owl:qualifiedCardinality>
                <owl:onDataRange rdf:resource="http://www.w3.org/2001/XMLSchema#double"/>
            </owl:Restriction>
        </rdfs:subClassOf>
        <rdfs:comment xml:lang="en">(Euclidean) vector is used to represent quantities that both magnitude and direction.</rdfs:comment>
        <rdfs:label xml:lang="en">Vector</rdfs:label>
        <skos:defintion xml:lang="en">(Euclidean) vector used to represent quantities that both magnitude and direction.</skos:defintion>
    </owl:Class>
    


    <!-- https://purls.helmholtz-metadaten.de/disos/cso#VectorComponentOfBasis -->

    <owl:Class rdf:about="https://purls.helmholtz-metadaten.de/disos/cso#VectorComponentOfBasis">
        <rdfs:subClassOf rdf:resource="http://qudt.org/schema/qudt/Quantity"/>
        <rdfs:subClassOf>
            <owl:Class>
                <owl:intersectionOf rdf:parseType="Collection">
                    <owl:Restriction>
                        <owl:onProperty rdf:resource="https://purls.helmholtz-metadaten.de/disos/cso#hasBasis"/>
                        <owl:someValuesFrom rdf:resource="https://w3id.org/mdo/structure/Basis"/>
                    </owl:Restriction>
                    <owl:Restriction>
                        <owl:onProperty rdf:resource="https://purls.helmholtz-metadaten.de/disos/cso#hasBasis"/>
                        <owl:allValuesFrom rdf:resource="https://w3id.org/mdo/structure/Basis"/>
                    </owl:Restriction>
                </owl:intersectionOf>
            </owl:Class>
        </rdfs:subClassOf>
        <rdfs:subClassOf>
            <owl:Class>
                <owl:intersectionOf rdf:parseType="Collection">
                    <owl:Restriction>
                        <owl:onProperty rdf:resource="https://purls.helmholtz-metadaten.de/disos/cso#firstAxisComponent"/>
                        <owl:qualifiedCardinality rdf:datatype="http://www.w3.org/2001/XMLSchema#nonNegativeInteger">1</owl:qualifiedCardinality>
                        <owl:onDataRange rdf:resource="http://www.w3.org/2001/XMLSchema#double"/>
                    </owl:Restriction>
                    <owl:Restriction>
                        <owl:onProperty rdf:resource="https://purls.helmholtz-metadaten.de/disos/cso#secondAxisComponent"/>
                        <owl:qualifiedCardinality rdf:datatype="http://www.w3.org/2001/XMLSchema#nonNegativeInteger">1</owl:qualifiedCardinality>
                        <owl:onDataRange rdf:resource="http://www.w3.org/2001/XMLSchema#double"/>
                    </owl:Restriction>
                    <owl:Restriction>
                        <owl:onProperty rdf:resource="https://purls.helmholtz-metadaten.de/disos/cso#thirdAxisComponent"/>
                        <owl:qualifiedCardinality rdf:datatype="http://www.w3.org/2001/XMLSchema#nonNegativeInteger">1</owl:qualifiedCardinality>
                        <owl:onDataRange rdf:resource="http://www.w3.org/2001/XMLSchema#double"/>
                    </owl:Restriction>
                </owl:intersectionOf>
            </owl:Class>
        </rdfs:subClassOf>
        <rdfs:comment xml:lang="en">Vector components/vector coordinates of particular basis. It has relation to a specific basis.</rdfs:comment>
        <rdfs:label xml:lang="en">Vector Component of Basis</rdfs:label>
    </owl:Class>
    


    <!-- https://purls.helmholtz-metadaten.de/disos/diso#BurgersVector -->

    <owl:Class rdf:about="https://purls.helmholtz-metadaten.de/disos/diso#BurgersVector">
        <rdfs:subClassOf rdf:resource="https://purls.helmholtz-metadaten.de/disos/cso#Vector"/>
        <rdfs:comment xml:lang="en">An elementary unit (length order of lattice parameter) of lattice translation. The basic notion of the Burgers vector comes from the closure failure of an initially perfect lattice due to the existence of dislocation. The magnitude and direction of closure failure are characterized by the Burgers vector.</rdfs:comment>
        <rdfs:comment xml:lang="de">Eine elementare Einheit (Lngenordnung der Gitterparameter) der Gittertranslation. Der grundlegende Begriff des Burgers-Vektors leitet sich aus dem Versagen der Schlieung eines ursprnglich perfekten Gitters aufgrund der Existenz von Versetzungen ab. Das Ausma und die Richtung des Schliefehlers werden durch den Burgers-Vektor charakterisiert.</rdfs:comment>
        <rdfs:label xml:lang="en">Burgers Vector</rdfs:label>
        <rdfs:label xml:lang="de">der Burgersvektor</rdfs:label>
    </owl:Class>
    


    <!-- https://purls.helmholtz-metadaten.de/disos/diso#DDDSimulation -->

    <owl:Class rdf:about="https://purls.helmholtz-metadaten.de/disos/diso#DDDSimulation">
        <rdfs:subClassOf rdf:resource="http://www.w3.org/ns/prov#Activity"/>
        <rdfs:subClassOf rdf:resource="https://w3id.org/mdo/core/Calculation"/>
        <rdfs:subClassOf>
            <owl:Class>
                <owl:intersectionOf rdf:parseType="Collection">
                    <owl:Restriction>
                        <owl:onProperty rdf:resource="https://purls.helmholtz-metadaten.de/disos/diso#hasInputDislocationStructure"/>
                        <owl:someValuesFrom rdf:resource="https://purls.helmholtz-metadaten.de/disos/diso#DislocationStructure"/>
                    </owl:Restriction>
                    <owl:Restriction>
                        <owl:onProperty rdf:resource="https://purls.helmholtz-metadaten.de/disos/diso#hasInputDislocationStructure"/>
                        <owl:allValuesFrom rdf:resource="https://purls.helmholtz-metadaten.de/disos/diso#DislocationStructure"/>
                    </owl:Restriction>
                    <owl:Restriction>
                        <owl:onProperty rdf:resource="https://purls.helmholtz-metadaten.de/disos/diso#hasOutputDislocationStructure"/>
                        <owl:allValuesFrom rdf:resource="https://purls.helmholtz-metadaten.de/disos/diso#DislocationStructure"/>
                    </owl:Restriction>
                </owl:intersectionOf>
            </owl:Class>
        </rdfs:subClassOf>
        <rdfs:subClassOf>
            <owl:Restriction>
                <owl:onProperty rdf:resource="http://www.w3.org/ns/prov#wasAssociatedWith"/>
                <owl:someValuesFrom rdf:resource="http://www.w3.org/ns/prov#Person"/>
            </owl:Restriction>
        </rdfs:subClassOf>
    </owl:Class>
    


    <!-- https://purls.helmholtz-metadaten.de/disos/diso#DiscretizedLine -->

    <owl:Class rdf:about="https://purls.helmholtz-metadaten.de/disos/diso#DiscretizedLine">
        <rdfs:subClassOf rdf:resource="http://emmo.info/emmo#EMMO_4ce76d7f_03f8_45b6_9003_90052a79bfaa"/>
        <rdfs:subClassOf>
            <owl:Restriction>
                <owl:onProperty rdf:resource="https://purls.helmholtz-metadaten.de/disos/diso#hasSegment"/>
                <owl:allValuesFrom rdf:resource="https://purls.helmholtz-metadaten.de/disos/diso#Segment"/>
            </owl:Restriction>
        </rdfs:subClassOf>
        <rdfs:subClassOf>
            <owl:Restriction>
                <owl:onProperty rdf:resource="https://purls.helmholtz-metadaten.de/disos/diso#hasShapeFunction"/>
                <owl:allValuesFrom rdf:resource="https://purls.helmholtz-metadaten.de/disos/diso#ShapeFunction"/>
            </owl:Restriction>
        </rdfs:subClassOf>
        <rdfs:subClassOf>
            <owl:Restriction>
                <owl:onProperty rdf:resource="https://purls.helmholtz-metadaten.de/disos/diso#slipArea"/>
                <owl:qualifiedCardinality rdf:datatype="http://www.w3.org/2001/XMLSchema#nonNegativeInteger">1</owl:qualifiedCardinality>
                <owl:onDataRange rdf:resource="http://www.w3.org/2001/XMLSchema#double"/>
            </owl:Restriction>
        </rdfs:subClassOf>
        <owl:disjointWith rdf:resource="https://purls.helmholtz-metadaten.de/disos/diso#Line"/>
        <rdfs:comment xml:lang="de">Die numerische Darstellung der Versetzungslinie, die in die Anzahl der Segmente diskretisiert ist.</rdfs:comment>
        <rdfs:comment xml:lang="en">The numerical representation of the dislocation line that is discretized into the number of segments.</rdfs:comment>
        <rdfs:label xml:lang="en">Discretized Line</rdfs:label>
        <rdfs:label xml:lang="de">die Diskretisierte Linie</rdfs:label>
    </owl:Class>
    


    <!-- https://purls.helmholtz-metadaten.de/disos/diso#Dislocation -->

    <owl:Class rdf:about="https://purls.helmholtz-metadaten.de/disos/diso#Dislocation">
        <rdfs:subClassOf rdf:resource="https://purls.helmholtz-metadaten.de/disos/diso#LineDefect"/>
        <rdfs:subClassOf>
            <owl:Class>
                <owl:intersectionOf rdf:parseType="Collection">
                    <owl:Restriction>
                        <owl:onProperty rdf:resource="https://purls.helmholtz-metadaten.de/disos/diso#hasBurgersVector"/>
                        <owl:someValuesFrom rdf:resource="https://purls.helmholtz-metadaten.de/disos/diso#BurgersVector"/>
                    </owl:Restriction>
                    <owl:Restriction>
                        <owl:onProperty rdf:resource="https://purls.helmholtz-metadaten.de/disos/diso#hasBurgersVector"/>
                        <owl:allValuesFrom rdf:resource="https://purls.helmholtz-metadaten.de/disos/diso#BurgersVector"/>
                    </owl:Restriction>
                </owl:intersectionOf>
            </owl:Class>
        </rdfs:subClassOf>
        <rdfs:subClassOf>
            <owl:Class>
                <owl:intersectionOf rdf:parseType="Collection">
                    <owl:Restriction>
                        <owl:onProperty rdf:resource="https://purls.helmholtz-metadaten.de/disos/diso#hasLineSense"/>
                        <owl:someValuesFrom rdf:resource="https://purls.helmholtz-metadaten.de/disos/diso#LineSense"/>
                    </owl:Restriction>
                    <owl:Restriction>
                        <owl:onProperty rdf:resource="https://purls.helmholtz-metadaten.de/disos/diso#hasLineSense"/>
                        <owl:allValuesFrom rdf:resource="https://purls.helmholtz-metadaten.de/disos/diso#LineSense"/>
                    </owl:Restriction>
                </owl:intersectionOf>
            </owl:Class>
        </rdfs:subClassOf>
        <rdfs:subClassOf>
            <owl:Restriction>
                <owl:onProperty rdf:resource="https://purls.helmholtz-metadaten.de/disos/diso#hasMathematicalRepresentation"/>
                <owl:someValuesFrom rdf:resource="https://purls.helmholtz-metadaten.de/disos/diso#Line"/>
            </owl:Restriction>
        </rdfs:subClassOf>
        <rdfs:subClassOf>
            <owl:Restriction>
                <owl:onProperty rdf:resource="https://purls.helmholtz-metadaten.de/disos/diso#movesOn"/>
                <owl:someValuesFrom rdf:resource="https://purls.helmholtz-metadaten.de/disos/diso#SlipPlane"/>
            </owl:Restriction>
        </rdfs:subClassOf>
        <rdfs:subClassOf>
            <owl:Restriction>
                <owl:onProperty rdf:resource="https://purls.helmholtz-metadaten.de/disos/diso#observedBy"/>
                <owl:someValuesFrom rdf:resource="https://purls.helmholtz-metadaten.de/disos/diso#FieldIonMicroscopy"/>
            </owl:Restriction>
        </rdfs:subClassOf>
        <rdfs:subClassOf>
            <owl:Restriction>
                <owl:onProperty rdf:resource="https://purls.helmholtz-metadaten.de/disos/diso#observedBy"/>
                <owl:someValuesFrom rdf:resource="https://purls.helmholtz-metadaten.de/disos/diso#TransmissionElectronMicroscopy"/>
            </owl:Restriction>
        </rdfs:subClassOf>
        <rdfs:subClassOf>
            <owl:Restriction>
                <owl:onProperty rdf:resource="https://purls.helmholtz-metadaten.de/disos/diso#resultsIn"/>
                <owl:someValuesFrom rdf:resource="https://purls.helmholtz-metadaten.de/disos/diso#LatticeDisplacement"/>
            </owl:Restriction>
        </rdfs:subClassOf>
        <rdfs:comment xml:lang="de">Ein linearer oder eindimensionaler Defekt, um den herum einige der Atome falsch ausgerichtet sind. Im Mesoscale ist eine Versetzung ein linienfrmiges Objekt, das eine Grenze darstellt, die die Regionen auf der Gleitebene, in denen ein Gleiten stattgefunden hat, von denen trennt, in denen dies nicht der Fall war.</rdfs:comment>
        <rdfs:comment xml:lang="en">Linear or one-dimensional defect around which some of the atoms are misaligned. In the mesoscale, a dislocation is a line object that is a boundary separating the regions on the slip plane which have undergone slip from those that have not.</rdfs:comment>
        <rdfs:comment xml:lang="en">The presence of dislocation introduces local disturbance of the atomic-level geometry.</rdfs:comment>
        <rdfs:label xml:lang="en">Dislocation</rdfs:label>
        <rdfs:label xml:lang="de">die Versetzung</rdfs:label>
    </owl:Class>
    


    <!-- https://purls.helmholtz-metadaten.de/disos/diso#DislocationStructure -->

    <owl:Class rdf:about="https://purls.helmholtz-metadaten.de/disos/diso#DislocationStructure">
        <rdfs:subClassOf rdf:resource="https://w3id.org/mdo/core/Structure"/>
        <rdfs:subClassOf>
            <owl:Class>
                <owl:intersectionOf rdf:parseType="Collection">
                    <owl:Restriction>
                        <owl:onProperty rdf:resource="https://purls.helmholtz-metadaten.de/disos/cdo#hasCrystallographicDefect"/>
                        <owl:someValuesFrom rdf:resource="https://purls.helmholtz-metadaten.de/disos/diso#Dislocation"/>
                    </owl:Restriction>
                    <owl:Restriction>
                        <owl:onProperty rdf:resource="https://purls.helmholtz-metadaten.de/disos/cdo#hasCrystallographicDefect"/>
                        <owl:allValuesFrom rdf:resource="https://purls.helmholtz-metadaten.de/disos/diso#Dislocation"/>
                    </owl:Restriction>
                </owl:intersectionOf>
            </owl:Class>
        </rdfs:subClassOf>
        <rdfs:subClassOf>
            <owl:Class>
                <owl:intersectionOf rdf:parseType="Collection">
                    <owl:Restriction>
                        <owl:onProperty rdf:resource="https://purls.helmholtz-metadaten.de/disos/diso#relatesToCrystallineMaterial"/>
                        <owl:someValuesFrom rdf:resource="https://purls.helmholtz-metadaten.de/disos/cdo#CrystallineMaterial"/>
                    </owl:Restriction>
                    <owl:Restriction>
                        <owl:onProperty rdf:resource="https://purls.helmholtz-metadaten.de/disos/diso#relatesToCrystallineMaterial"/>
                        <owl:allValuesFrom rdf:resource="https://purls.helmholtz-metadaten.de/disos/cdo#CrystallineMaterial"/>
                    </owl:Restriction>
                </owl:intersectionOf>
            </owl:Class>
        </rdfs:subClassOf>
    </owl:Class>
    


    <!-- https://purls.helmholtz-metadaten.de/disos/diso#EdgeDislocation -->

    <owl:Class rdf:about="https://purls.helmholtz-metadaten.de/disos/diso#EdgeDislocation">
        <rdfs:subClassOf rdf:resource="https://purls.helmholtz-metadaten.de/disos/diso#Dislocation"/>
        <owl:disjointWith rdf:resource="https://purls.helmholtz-metadaten.de/disos/diso#ScrewDislocation"/>
        <rdfs:comment xml:lang="en">A dislocation that has a line sense perpendicular to its Burgers vector.</rdfs:comment>
        <rdfs:comment xml:lang="de">Eine Versetzung, die Burgersvektor und Versetzungslinie stehen senkrecht zueinander</rdfs:comment>
        <rdfs:label xml:lang="en">Edge Dislocation</rdfs:label>
        <rdfs:label xml:lang="de">die Stufenversetzung</rdfs:label>
    </owl:Class>
    


    <!-- https://purls.helmholtz-metadaten.de/disos/diso#FamilyOfCrystalDirection -->

    <owl:Class rdf:about="https://purls.helmholtz-metadaten.de/disos/diso#FamilyOfCrystalDirection">
        <rdfs:subClassOf>
            <owl:Restriction>
                <owl:onProperty rdf:resource="https://purls.helmholtz-metadaten.de/disos/diso#familyDirectionMillerIndice"/>
                <owl:qualifiedCardinality rdf:datatype="http://www.w3.org/2001/XMLSchema#nonNegativeInteger">1</owl:qualifiedCardinality>
                <owl:onDataRange rdf:resource="http://www.w3.org/2001/XMLSchema#string"/>
            </owl:Restriction>
        </rdfs:subClassOf>
        <owl:disjointWith rdf:resource="https://purls.helmholtz-metadaten.de/disos/diso#FamilyOfCrystalPlane"/>
        <rdfs:comment xml:lang="en">A set of symmetrically equivalent directions in the lattice.</rdfs:comment>
        <rdfs:comment xml:lang="de">die Menge aller symmetrisch quivalenten Richtungen.</rdfs:comment>
        <rdfs:label xml:lang="en">Family of Crystal Direction</rdfs:label>
        <rdfs:label xml:lang="de">die Familie der Gitterrichtung</rdfs:label>
    </owl:Class>
    


    <!-- https://purls.helmholtz-metadaten.de/disos/diso#FamilyOfCrystalPlane -->

    <owl:Class rdf:about="https://purls.helmholtz-metadaten.de/disos/diso#FamilyOfCrystalPlane">
        <rdfs:subClassOf>
            <owl:Restriction>
                <owl:onProperty rdf:resource="https://purls.helmholtz-metadaten.de/disos/diso#familyPlaneMillerIndice"/>
                <owl:qualifiedCardinality rdf:datatype="http://www.w3.org/2001/XMLSchema#nonNegativeInteger">1</owl:qualifiedCardinality>
                <owl:onDataRange rdf:resource="http://www.w3.org/2001/XMLSchema#string"/>
            </owl:Restriction>
        </rdfs:subClassOf>
        <rdfs:comment xml:lang="en">A set of symmetrically equivalent planes in the lattice.</rdfs:comment>
        <rdfs:comment xml:lang="de">Steht fr Kristallformen, d. h. die Menge aller symmetrisch quivalenten Flchen.</rdfs:comment>
        <rdfs:label xml:lang="en">Family of Crystal Plane</rdfs:label>
        <rdfs:label xml:lang="de">die Familie der Gitterebene</rdfs:label>
    </owl:Class>
    


    <!-- https://purls.helmholtz-metadaten.de/disos/diso#FieldIonMicroscopy -->

    <owl:Class rdf:about="https://purls.helmholtz-metadaten.de/disos/diso#FieldIonMicroscopy">
        <owl:disjointWith rdf:resource="https://purls.helmholtz-metadaten.de/disos/diso#TransmissionElectronMicroscopy"/>
        <rdfs:comment xml:lang="de">Die Feldionenmikroskopie (FIM) ist eine Mikroskopietechnik, mit der sich die Anordnung von Atomen abbilden lsst.</rdfs:comment>
        <rdfs:comment xml:lang="en">Field Ion Microscopy (FIM) is a microscopy technique that can be used to image the arrangement of atoms.</rdfs:comment>
        <rdfs:label xml:lang="de">Das Feldionenmikroskop</rdfs:label>
        <rdfs:label xml:lang="en">Field Ion Microscopy</rdfs:label>
    </owl:Class>
    


    <!-- https://purls.helmholtz-metadaten.de/disos/diso#LatticeDirection -->

    <owl:Class rdf:about="https://purls.helmholtz-metadaten.de/disos/diso#LatticeDirection">
        <rdfs:subClassOf rdf:resource="https://purls.helmholtz-metadaten.de/disos/cso#Vector"/>
        <rdfs:subClassOf rdf:resource="https://purls.helmholtz-metadaten.de/disos/diso#FamilyOfCrystalDirection"/>
        <rdfs:subClassOf>
            <owl:Class>
                <owl:intersectionOf rdf:parseType="Collection">
                    <owl:Restriction>
                        <owl:onProperty rdf:resource="https://purls.helmholtz-metadaten.de/disos/diso#hasLatticePoint"/>
                        <owl:someValuesFrom rdf:resource="https://purls.helmholtz-metadaten.de/disos/diso#LatticePoint"/>
                    </owl:Restriction>
                    <owl:Restriction>
                        <owl:onProperty rdf:resource="https://purls.helmholtz-metadaten.de/disos/diso#hasLatticePoint"/>
                        <owl:allValuesFrom rdf:resource="https://purls.helmholtz-metadaten.de/disos/diso#LatticePoint"/>
                    </owl:Restriction>
                </owl:intersectionOf>
            </owl:Class>
        </rdfs:subClassOf>
        <rdfs:subClassOf>
            <owl:Restriction>
                <owl:onProperty rdf:resource="https://purls.helmholtz-metadaten.de/disos/diso#directionMillerIndice"/>
                <owl:qualifiedCardinality rdf:datatype="http://www.w3.org/2001/XMLSchema#nonNegativeInteger">1</owl:qualifiedCardinality>
                <owl:onDataRange rdf:resource="http://www.w3.org/2001/XMLSchema#string"/>
            </owl:Restriction>
        </rdfs:subClassOf>
        <rdfs:comment xml:lang="de">Die Vektorrichtung innerhalb des Gitters, die zwei Gitterpunkte verbindet.</rdfs:comment>
        <rdfs:comment xml:lang="en">The vector direction inside the lattice that is connecting two lattice points.</rdfs:comment>
        <rdfs:label xml:lang="de">Die Gitterrichtung</rdfs:label>
        <rdfs:label xml:lang="en">Lattice Direction</rdfs:label>
    </owl:Class>
    


    <!-- https://purls.helmholtz-metadaten.de/disos/diso#LatticeDisplacement -->

    <owl:Class rdf:about="https://purls.helmholtz-metadaten.de/disos/diso#LatticeDisplacement">
        <rdfs:comment xml:lang="de">Die Verschiebung von Atomen von ihren perfekten Gitterpunkt aufgrund des Fehlens von Defekten, z. B. Punktuelle Defekte, Linearedefekte und Korngrenzen.</rdfs:comment>
        <rdfs:comment xml:lang="en">The displacement of atoms from their perfect lattice sites due to the existence of defects, e.g., point defect, line defect, and grain boundary.</rdfs:comment>
        <rdfs:label xml:lang="en">Lattice Displacement</rdfs:label>
        <rdfs:label xml:lang="de">die Verschiebung</rdfs:label>
    </owl:Class>
    


    <!-- https://purls.helmholtz-metadaten.de/disos/diso#LatticePlane -->

    <owl:Class rdf:about="https://purls.helmholtz-metadaten.de/disos/diso#LatticePlane">
        <rdfs:subClassOf rdf:resource="https://purls.helmholtz-metadaten.de/disos/diso#FamilyOfCrystalPlane"/>
        <rdfs:subClassOf>
            <owl:Class>
                <owl:intersectionOf rdf:parseType="Collection">
                    <owl:Restriction>
                        <owl:onProperty rdf:resource="https://purls.helmholtz-metadaten.de/disos/diso#hasLatticeDirection"/>
                        <owl:someValuesFrom rdf:resource="https://purls.helmholtz-metadaten.de/disos/diso#LatticeDirection"/>
                    </owl:Restriction>
                    <owl:Restriction>
                        <owl:onProperty rdf:resource="https://purls.helmholtz-metadaten.de/disos/diso#hasLatticeDirection"/>
                        <owl:allValuesFrom rdf:resource="https://purls.helmholtz-metadaten.de/disos/diso#LatticeDirection"/>
                    </owl:Restriction>
                </owl:intersectionOf>
            </owl:Class>
        </rdfs:subClassOf>
        <rdfs:subClassOf>
            <owl:Class>
                <owl:intersectionOf rdf:parseType="Collection">
                    <owl:Restriction>
                        <owl:onProperty rdf:resource="https://purls.helmholtz-metadaten.de/disos/diso#hasLatticePoint"/>
                        <owl:someValuesFrom rdf:resource="https://purls.helmholtz-metadaten.de/disos/diso#LatticePoint"/>
                    </owl:Restriction>
                    <owl:Restriction>
                        <owl:onProperty rdf:resource="https://purls.helmholtz-metadaten.de/disos/diso#hasLatticePoint"/>
                        <owl:allValuesFrom rdf:resource="https://purls.helmholtz-metadaten.de/disos/diso#LatticePoint"/>
                    </owl:Restriction>
                </owl:intersectionOf>
            </owl:Class>
        </rdfs:subClassOf>
        <rdfs:subClassOf>
            <owl:Restriction>
                <owl:onProperty rdf:resource="https://purls.helmholtz-metadaten.de/disos/diso#hasVectorOrigin"/>
                <owl:allValuesFrom rdf:resource="https://purls.helmholtz-metadaten.de/disos/diso#VectorOrigin"/>
            </owl:Restriction>
        </rdfs:subClassOf>
        <rdfs:subClassOf>
            <owl:Restriction>
                <owl:onProperty rdf:resource="https://purls.helmholtz-metadaten.de/disos/diso#planeMillerIndice"/>
                <owl:qualifiedCardinality rdf:datatype="http://www.w3.org/2001/XMLSchema#nonNegativeInteger">1</owl:qualifiedCardinality>
                <owl:onDataRange rdf:resource="http://www.w3.org/2001/XMLSchema#string"/>
            </owl:Restriction>
        </rdfs:subClassOf>
        <rdfs:comment xml:lang="de">Die Gitterebene bildet eine unendlich gestreckte Ebene (gekennzeichnet durch eine Ebenennormale), die die Gitterpunkte so schneidet, dass wiederum eine regelmige Anordnung der Gitterpunkte in der Ebene entsteht.</rdfs:comment>
        <rdfs:comment xml:lang="en">The lattice plane forms an infinitely stretched plane (characterized through a plane normal) that cuts through lattice points such that, again, a regular arrangement of lattice points in the plane occurs.</rdfs:comment>
        <rdfs:label xml:lang="en">Lattice Plane</rdfs:label>
        <rdfs:label xml:lang="de">die Gitterebene</rdfs:label>
    </owl:Class>
    


    <!-- https://purls.helmholtz-metadaten.de/disos/diso#LatticePoint -->

    <owl:Class rdf:about="https://purls.helmholtz-metadaten.de/disos/diso#LatticePoint">
        <rdfs:subClassOf rdf:resource="https://purls.helmholtz-metadaten.de/disos/cso#Point"/>
        <rdfs:comment xml:lang="de">Der Gitterpunkt ist der Punkt, an dem sich ein Atom oder ein Molekl befindet.</rdfs:comment>
        <rdfs:comment xml:lang="en">Lattice point is the point where atom(s) or molecule(s) is located.</rdfs:comment>
        <rdfs:label xml:lang="en">Lattice Point</rdfs:label>
        <rdfs:label xml:lang="de">der Gitterpunkt</rdfs:label>
    </owl:Class>
    


    <!-- https://purls.helmholtz-metadaten.de/disos/diso#Line -->

    <owl:Class rdf:about="https://purls.helmholtz-metadaten.de/disos/diso#Line">
        <rdfs:subClassOf rdf:resource="http://emmo.info/emmo#EMMO_f7ed665b_c2e1_42bc_889b_6b42ed3a36f0"/>
        <rdfs:subClassOf>
            <owl:Restriction>
                <owl:onProperty rdf:resource="https://purls.helmholtz-metadaten.de/disos/diso#hasNumericalRepresentation"/>
                <owl:someValuesFrom rdf:resource="https://purls.helmholtz-metadaten.de/disos/diso#DiscretizedLine"/>
            </owl:Restriction>
        </rdfs:subClassOf>
        <owl:disjointWith rdf:resource="https://purls.helmholtz-metadaten.de/disos/diso#Node"/>
        <rdfs:comment xml:lang="en">Mathematical representation of dislocation as &apos;Line&apos;. An instance of mathematical representation of a dislocation line is an oriented curve parameterized by its arc length.</rdfs:comment>
        <rdfs:comment xml:lang="de">Mathematische Darstellung der Versetzung als &quot;Linie&quot;. Ein Beispiel fr die mathematische Darstellung einer Versetzungslinie ist eine orientierte Kurve, die durch ihre Bogenlnge parametrisiert ist.</rdfs:comment>
        <rdfs:label xml:lang="en">Line</rdfs:label>
        <rdfs:label xml:lang="de">die Linie</rdfs:label>
    </owl:Class>
    


    <!-- https://purls.helmholtz-metadaten.de/disos/diso#LineDefect -->

    <owl:Class rdf:about="https://purls.helmholtz-metadaten.de/disos/diso#LineDefect">
        <rdfs:subClassOf rdf:resource="https://purls.helmholtz-metadaten.de/disos/cdo#CrystallographicDefect"/>
        <rdfs:comment xml:lang="en">Linear or one-dimensional defect around which some of the atoms are misaligned.</rdfs:comment>
        <rdfs:comment xml:lang="de">Linearer oder eindimensionaler Defekt, um den herum einige Atome falsch ausgerichtet sind.</rdfs:comment>
        <rdfs:label xml:lang="en">Line Defect</rdfs:label>
        <rdfs:label xml:lang="de">der linienhafter Defekt</rdfs:label>
    </owl:Class>
    


    <!-- https://purls.helmholtz-metadaten.de/disos/diso#LineSense -->

    <owl:Class rdf:about="https://purls.helmholtz-metadaten.de/disos/diso#LineSense">
        <rdfs:comment xml:lang="en">A sense that characterizes a directed line, i.e., it has a start and an end.</rdfs:comment>
        <rdfs:comment xml:lang="de">Ein Element, das eine gerichtete Linie charakterisiert, d. h. sie hat einen Anfang und ein Ende.</rdfs:comment>
        <rdfs:label xml:lang="en">Line Sense</rdfs:label>
        <rdfs:label xml:lang="de">die Versetzunglinie</rdfs:label>
    </owl:Class>
    


    <!-- https://purls.helmholtz-metadaten.de/disos/diso#Node -->

    <owl:Class rdf:about="https://purls.helmholtz-metadaten.de/disos/diso#Node">
        <rdfs:subClassOf rdf:resource="https://purls.helmholtz-metadaten.de/disos/cso#Point"/>
        <owl:disjointWith rdf:resource="https://purls.helmholtz-metadaten.de/disos/diso#Segment"/>
        <rdfs:comment xml:lang="en">A point of a segment.</rdfs:comment>
        <rdfs:comment xml:lang="de">Ein Punkt eines Segments.</rdfs:comment>
        <rdfs:label xml:lang="en">Node</rdfs:label>
        <rdfs:label xml:lang="de">der Knoten</rdfs:label>
    </owl:Class>
    


    <!-- https://purls.helmholtz-metadaten.de/disos/diso#ScrewDislocation -->

    <owl:Class rdf:about="https://purls.helmholtz-metadaten.de/disos/diso#ScrewDislocation">
        <rdfs:subClassOf rdf:resource="https://purls.helmholtz-metadaten.de/disos/diso#Dislocation"/>
        <rdfs:comment xml:lang="en">A dislocation that has a line sense parallel to its Burgers vector.</rdfs:comment>
        <rdfs:comment xml:lang="de">Eine Versetzung, die Burgersvektor und Versetzungslinie liegen parallel.</rdfs:comment>
        <rdfs:label xml:lang="en">Screw Dislocation</rdfs:label>
        <rdfs:label xml:lang="de">die Schraubenversetzung</rdfs:label>
    </owl:Class>
    


    <!-- https://purls.helmholtz-metadaten.de/disos/diso#Segment -->

    <owl:Class rdf:about="https://purls.helmholtz-metadaten.de/disos/diso#Segment">
        <rdfs:subClassOf>
            <owl:Restriction>
                <owl:onProperty rdf:resource="https://purls.helmholtz-metadaten.de/disos/diso#hasEndNode"/>
                <owl:allValuesFrom rdf:resource="https://purls.helmholtz-metadaten.de/disos/diso#Node"/>
            </owl:Restriction>
        </rdfs:subClassOf>
        <rdfs:subClassOf>
            <owl:Restriction>
                <owl:onProperty rdf:resource="https://purls.helmholtz-metadaten.de/disos/diso#hasStartNode"/>
                <owl:allValuesFrom rdf:resource="https://purls.helmholtz-metadaten.de/disos/diso#Node"/>
            </owl:Restriction>
        </rdfs:subClassOf>
        <rdfs:subClassOf>
            <owl:Restriction>
                <owl:onProperty rdf:resource="https://purls.helmholtz-metadaten.de/disos/diso#isSegmentOf"/>
                <owl:allValuesFrom rdf:resource="https://purls.helmholtz-metadaten.de/disos/diso#DiscretizedLine"/>
            </owl:Restriction>
        </rdfs:subClassOf>
        <rdfs:comment xml:lang="de">Das Segment ist ein Teil einer Linie, der von zwei bestimmten Endpunkten begrenzt wird und Punkte auf der Linie zwischen den Endpunkten enthalten kann.</rdfs:comment>
        <rdfs:comment xml:lang="en">The segment is a part of a line bounded by two distinct end points and may contain points on the line between its endpoints.</rdfs:comment>
        <rdfs:label xml:lang="en">Segment</rdfs:label>
        <rdfs:label xml:lang="de">die Strecke</rdfs:label>
    </owl:Class>
    


    <!-- https://purls.helmholtz-metadaten.de/disos/diso#ShapeFunction -->

    <owl:Class rdf:about="https://purls.helmholtz-metadaten.de/disos/diso#ShapeFunction">
        <rdfs:comment xml:lang="de">Die Formfunktion ist die Funktion, die die Lsung zwischen den an den Netzknoten erhaltenen diskreten Werten interpoliert. Bei der diskretisierten Versetzung bestimmt die Formfunktion die Form eines Segments und letztlich die Form der Linie. Beispiele fr Formfunktionen, die zur Diskretisierung der Versetzung verwendet werden, sind kreisfrmig, elliptisch, spiralfrmig, linear, kubisch und quintisch.</rdfs:comment>
        <rdfs:comment xml:lang="en">The shape function is the function that interpolates the solution between the discrete values obtained at the mesh nodes. In discretized dislocation, the shape function determines the shape of a segment and ultimately determines the shape of the line. Examples of shape function that is used to discretize the dislocation are circular, elliptic, spiral, linear, cubic, and quintic.</rdfs:comment>
        <rdfs:label xml:lang="en">Shape Function</rdfs:label>
        <rdfs:label xml:lang="de">die Formfunktion</rdfs:label>
    </owl:Class>
    


    <!-- https://purls.helmholtz-metadaten.de/disos/diso#SlipDirection -->

    <owl:Class rdf:about="https://purls.helmholtz-metadaten.de/disos/diso#SlipDirection">
        <rdfs:subClassOf rdf:resource="https://purls.helmholtz-metadaten.de/disos/diso#LatticeDirection"/>
        <rdfs:comment xml:lang="de">Die Richtung in der Gleitebene, in der die plastische Verformung stattfindet. Die Gleitrichtung entspricht einem der krzesten Translationsvektoren des Gitters.</rdfs:comment>
        <rdfs:comment xml:lang="en">The direction in the slip plane along which plastic deformation takes place. The slip direction corresponds to one of the shortest lattice translation vectors.</rdfs:comment>
        <rdfs:label xml:lang="en">Slip Direction</rdfs:label>
        <rdfs:label xml:lang="de">die Gleitrichtung</rdfs:label>
    </owl:Class>
    


    <!-- https://purls.helmholtz-metadaten.de/disos/diso#SlipPlane -->

    <owl:Class rdf:about="https://purls.helmholtz-metadaten.de/disos/diso#SlipPlane">
        <rdfs:subClassOf rdf:resource="https://purls.helmholtz-metadaten.de/disos/diso#LatticePlane"/>
        <rdfs:subClassOf>
            <owl:Class>
                <owl:intersectionOf rdf:parseType="Collection">
                    <owl:Restriction>
                        <owl:onProperty rdf:resource="https://purls.helmholtz-metadaten.de/disos/diso#hasSlipDirection"/>
                        <owl:someValuesFrom rdf:resource="https://purls.helmholtz-metadaten.de/disos/diso#SlipDirection"/>
                    </owl:Restriction>
                    <owl:Restriction>
                        <owl:onProperty rdf:resource="https://purls.helmholtz-metadaten.de/disos/diso#hasSlipDirection"/>
                        <owl:allValuesFrom rdf:resource="https://purls.helmholtz-metadaten.de/disos/diso#SlipDirection"/>
                    </owl:Restriction>
                </owl:intersectionOf>
            </owl:Class>
        </rdfs:subClassOf>
        <rdfs:subClassOf>
            <owl:Class>
                <owl:intersectionOf rdf:parseType="Collection">
                    <owl:Restriction>
                        <owl:onProperty rdf:resource="https://purls.helmholtz-metadaten.de/disos/diso#hasSlipPlaneNormal"/>
                        <owl:someValuesFrom rdf:resource="https://purls.helmholtz-metadaten.de/disos/diso#SlipPlaneNormal"/>
                    </owl:Restriction>
                    <owl:Restriction>
                        <owl:onProperty rdf:resource="https://purls.helmholtz-metadaten.de/disos/diso#hasSlipPlaneNormal"/>
                        <owl:allValuesFrom rdf:resource="https://purls.helmholtz-metadaten.de/disos/diso#SlipPlaneNormal"/>
                    </owl:Restriction>
                </owl:intersectionOf>
            </owl:Class>
        </rdfs:subClassOf>
        <rdfs:comment xml:lang="de">Die kristallografische/Gitterebene, entlang derer die Versetzungslinie verluft/bewegt wird. Die Gleitebene ist in der Regel die Ebene mit der hchsten Dichte an Atomen, d. h. mit dem grten Abstand.</rdfs:comment>
        <rdfs:comment xml:lang="en">The crystallographic/lattice plane along which the dislocation line traverses/moves. The slip plane is usually the plane with the highest density of atoms, i.e. most widely spaced.</rdfs:comment>
        <rdfs:label xml:lang="en">Slip Plane</rdfs:label>
        <rdfs:label xml:lang="de">die Gleitebene</rdfs:label>
    </owl:Class>
    


    <!-- https://purls.helmholtz-metadaten.de/disos/diso#SlipPlaneNormal -->

    <owl:Class rdf:about="https://purls.helmholtz-metadaten.de/disos/diso#SlipPlaneNormal">
        <rdfs:subClassOf rdf:resource="https://purls.helmholtz-metadaten.de/disos/cso#Vector"/>
        <rdfs:subClassOf>
            <owl:Restriction>
                <owl:onProperty rdf:resource="https://purls.helmholtz-metadaten.de/disos/diso#directionMillerIndice"/>
                <owl:qualifiedCardinality rdf:datatype="http://www.w3.org/2001/XMLSchema#nonNegativeInteger">1</owl:qualifiedCardinality>
                <owl:onDataRange rdf:resource="http://www.w3.org/2001/XMLSchema#string"/>
            </owl:Restriction>
        </rdfs:subClassOf>
        <rdfs:comment xml:lang="de">Der Einheitsnormalvektor der Gleitebenen.</rdfs:comment>
        <rdfs:comment xml:lang="en">The unit normal vector of slip planes.</rdfs:comment>
        <rdfs:label xml:lang="en">Slip Plane Normal</rdfs:label>
        <rdfs:label xml:lang="de">der Gleitebene Normalvektor</rdfs:label>
    </owl:Class>
    


    <!-- https://purls.helmholtz-metadaten.de/disos/diso#SlipSystem -->

    <owl:Class rdf:about="https://purls.helmholtz-metadaten.de/disos/diso#SlipSystem">
        <rdfs:subClassOf>
            <owl:Class>
                <owl:intersectionOf rdf:parseType="Collection">
                    <owl:Restriction>
                        <owl:onProperty rdf:resource="https://purls.helmholtz-metadaten.de/disos/diso#hasSlipDirection"/>
                        <owl:someValuesFrom rdf:resource="https://purls.helmholtz-metadaten.de/disos/diso#SlipDirection"/>
                    </owl:Restriction>
                    <owl:Restriction>
                        <owl:onProperty rdf:resource="https://purls.helmholtz-metadaten.de/disos/diso#hasSlipDirection"/>
                        <owl:allValuesFrom rdf:resource="https://purls.helmholtz-metadaten.de/disos/diso#SlipDirection"/>
                    </owl:Restriction>
                </owl:intersectionOf>
            </owl:Class>
        </rdfs:subClassOf>
        <rdfs:subClassOf>
            <owl:Class>
                <owl:intersectionOf rdf:parseType="Collection">
                    <owl:Restriction>
                        <owl:onProperty rdf:resource="https://purls.helmholtz-metadaten.de/disos/diso#hasSlipPlaneNormal"/>
                        <owl:someValuesFrom rdf:resource="https://purls.helmholtz-metadaten.de/disos/diso#SlipPlaneNormal"/>
                    </owl:Restriction>
                    <owl:Restriction>
                        <owl:onProperty rdf:resource="https://purls.helmholtz-metadaten.de/disos/diso#hasSlipPlaneNormal"/>
                        <owl:allValuesFrom rdf:resource="https://purls.helmholtz-metadaten.de/disos/diso#SlipPlaneNormal"/>
                    </owl:Restriction>
                </owl:intersectionOf>
            </owl:Class>
        </rdfs:subClassOf>
        <rdfs:comment xml:lang="en">A slip system is defined as the set of slip planes with the same unit normal vector and the same slip direction.</rdfs:comment>
        <rdfs:comment xml:lang="de">Ein Gleitsystem ist definiert als die Menge der Gleitebenen mit dem gleichen Einheitsnormalvektor und der gleichen Gleitrichtung.</rdfs:comment>
        <rdfs:label xml:lang="en">Slip System</rdfs:label>
        <rdfs:label xml:lang="de">das Gleitsystem</rdfs:label>
    </owl:Class>
    


    <!-- https://purls.helmholtz-metadaten.de/disos/diso#TransmissionElectronMicroscopy -->

    <owl:Class rdf:about="https://purls.helmholtz-metadaten.de/disos/diso#TransmissionElectronMicroscopy">
        <rdfs:comment xml:lang="de">Die Transmissionselektronenmikroskopie (TEM) ist eine Mikroskopietechnik, bei der ein Elektronenstrahl durch eine Probe geschickt wird, um ein Bild zu erzeugen. Bei der Probe handelt es sich hufig um einen ultradnnen Schnitt von weniger als 100 nm Dicke.</rdfs:comment>
        <rdfs:comment xml:lang="en">Transmission electron microscopy (TEM) is a microscopy technique in which a beam of electrons is transmitted through a specimen to form an image. The specimen is often an ultrathin section less than 100 nm thick.</rdfs:comment>
        <rdfs:label xml:lang="de">Die Transmissionselektronenmikroskopie</rdfs:label>
        <rdfs:label xml:lang="en">Transmission Electron Microscopy</rdfs:label>
    </owl:Class>
    


    <!-- https://purls.helmholtz-metadaten.de/disos/diso#VectorOrigin -->

    <owl:Class rdf:about="https://purls.helmholtz-metadaten.de/disos/diso#VectorOrigin">
        <rdfs:subClassOf rdf:resource="https://purls.helmholtz-metadaten.de/disos/cso#Point"/>
        <rdfs:comment xml:lang="en">A fixed point that is needed by the vector to identify other points in the space relative to its origin.</rdfs:comment>
        <rdfs:comment xml:lang="de">Ein Fixpunkt, der vom Vektor bentigt wird, um andere Punkte im Raum relativ zu seinem Ursprung zu identifizieren.</rdfs:comment>
        <rdfs:label xml:lang="en">Vector Origin</rdfs:label>
        <rdfs:label xml:lang="de">der Ursprung</rdfs:label>
    </owl:Class>
    


    <!-- https://w3id.org/mdo/core/Calculation -->

    <rdf:Description rdf:about="https://w3id.org/mdo/core/Calculation">
        <rdfs:subClassOf>
            <owl:Restriction>
                <owl:onProperty rdf:resource="http://www.w3.org/ns/prov#wasAssociatedWith"/>
                <owl:someValuesFrom rdf:resource="http://www.w3.org/ns/prov#SoftwareAgent"/>
            </owl:Restriction>
        </rdfs:subClassOf>
    </rdf:Description>
    


    <!-- https://w3id.org/mdo/structure/Basis -->

    <owl:Class rdf:about="https://w3id.org/mdo/structure/Basis">
        <rdfs:subClassOf>
            <owl:Restriction>
                <owl:onProperty rdf:resource="https://purls.helmholtz-metadaten.de/disos/cso#hasFirstAxisVector"/>
                <owl:qualifiedCardinality rdf:datatype="http://www.w3.org/2001/XMLSchema#nonNegativeInteger">1</owl:qualifiedCardinality>
                <owl:onClass rdf:resource="https://w3id.org/mdo/structure/CoordinateVector"/>
            </owl:Restriction>
        </rdfs:subClassOf>
        <rdfs:subClassOf>
            <owl:Restriction>
                <owl:onProperty rdf:resource="https://purls.helmholtz-metadaten.de/disos/cso#hasSecondAxisVector"/>
                <owl:qualifiedCardinality rdf:datatype="http://www.w3.org/2001/XMLSchema#nonNegativeInteger">1</owl:qualifiedCardinality>
                <owl:onClass rdf:resource="https://w3id.org/mdo/structure/CoordinateVector"/>
            </owl:Restriction>
        </rdfs:subClassOf>
        <rdfs:subClassOf>
            <owl:Restriction>
                <owl:onProperty rdf:resource="https://purls.helmholtz-metadaten.de/disos/cso#hasThirdAxisVector"/>
                <owl:qualifiedCardinality rdf:datatype="http://www.w3.org/2001/XMLSchema#nonNegativeInteger">1</owl:qualifiedCardinality>
                <owl:onClass rdf:resource="https://w3id.org/mdo/structure/CoordinateVector"/>
            </owl:Restriction>
        </rdfs:subClassOf>
        <rdfs:comment xml:lang="en">A basis defines a spatial unit used to express fractional coordinates.</rdfs:comment>
        <rdfs:label xml:lang="en">Basis</rdfs:label>
        <skos:defintion xml:lang="en">Set of vector(in 2-D two vectors and in 3-D three vectors) that linearly independent.</skos:defintion>
    </owl:Class>
    


    <!-- https://w3id.org/mdo/structure/CoordinateVector -->

    <owl:Class rdf:about="https://w3id.org/mdo/structure/CoordinateVector">
        <rdfs:subClassOf>
            <owl:Restriction>
                <owl:onProperty rdf:resource="https://w3id.org/mdo/structure/X_axisCoordinate"/>
                <owl:qualifiedCardinality rdf:datatype="http://www.w3.org/2001/XMLSchema#nonNegativeInteger">1</owl:qualifiedCardinality>
                <owl:onDataRange rdf:resource="http://www.w3.org/2001/XMLSchema#double"/>
            </owl:Restriction>
        </rdfs:subClassOf>
        <rdfs:subClassOf>
            <owl:Restriction>
                <owl:onProperty rdf:resource="https://w3id.org/mdo/structure/Y_axisCoordinate"/>
                <owl:qualifiedCardinality rdf:datatype="http://www.w3.org/2001/XMLSchema#nonNegativeInteger">1</owl:qualifiedCardinality>
                <owl:onDataRange rdf:resource="http://www.w3.org/2001/XMLSchema#double"/>
            </owl:Restriction>
        </rdfs:subClassOf>
        <rdfs:subClassOf>
            <owl:Restriction>
                <owl:onProperty rdf:resource="https://w3id.org/mdo/structure/Z_axisCoordinate"/>
                <owl:qualifiedCardinality rdf:datatype="http://www.w3.org/2001/XMLSchema#nonNegativeInteger">1</owl:qualifiedCardinality>
                <owl:onDataRange rdf:resource="http://www.w3.org/2001/XMLSchema#double"/>
            </owl:Restriction>
        </rdfs:subClassOf>
        <rdfs:label xml:lang="en">Coordinate Vector</rdfs:label>
        <skos:defintion xml:lang="en">A coordinate vector according to standard basis, i.e., e_x (1, 0, 0), e_y(0, 1, 0), and e_z (0, 0, 1).</skos:defintion>
    </owl:Class>
</rdf:RDF>



<!-- Generated by the OWL API (version 4.5.9.2019-02-01T07:24:44Z) https://github.com/owlcs/owlapi -->

